Port interference from SimAsm to ARMv8

ARMv8/ARMv8.thy
@@ -1,235 +1,41 @@
 theory ARMv8
-  imports ARMv8_State "../Syntax"
+  imports ARMv8_Exp "../Syntax"
 begin
 
 chapter \<open>ARMv8\<close>
-
-section \<open>Local Expression Language\<close>
-
-text \<open>
-Simple AST to represent expressions based on registers.
-Used to capture register operations and handle the implications of forwarding:
-the rewriting of expressions to enable additional reordering behaviours.
-
-Notably we include a tagged constant, the Glb, that represents a constant value that is
-dependent on a memory address. 
-This is necessary to capture the dependencies within a load operation.
-\<close>
-datatype ('v,'r) exp = Reg 'r | Val 'v | Glb 'v 'v | Exp "'v list \<Rightarrow> 'v" "('v,'r) exp list"
-
-text \<open>Evaluate an expression given a register state\<close>
-fun ev :: "('r \<Rightarrow> 'v) \<Rightarrow> ('v,'r) exp \<Rightarrow> 'v"
-  where 
-    "ev m (Reg r) = m r" | 
-    "ev _ (Val v) = v" |
-    "ev _ (Glb v _) = v" |
-    "ev m (Exp f rs) = f (map (ev m) rs)"
-
-text \<open>The syntactic register dependencies of an expression\<close>
-fun deps :: "('v,'r) exp \<Rightarrow> 'r set"
-  where 
-    "deps (Reg r) = {r}" |
-    "deps (Exp _ rs) = \<Union>(deps ` set rs)" |
-    "deps _ = {}"
-
-text \<open>The global dependencies of an expression\<close>
-fun glbs :: "('v,'r) exp \<Rightarrow> 'v set"
-  where
-    "glbs (Glb _ v) = {v}" |
-    "glbs (Exp _ rs) = \<Union>(glbs ` set rs)" |
-    "glbs _ = {}"
-
-text \<open>Substitute a register for an expression\<close>
-fun subst :: "('v,'r) exp \<Rightarrow> 'r \<Rightarrow> ('v,'r) exp \<Rightarrow> ('v,'r) exp"
-  where
-    "subst (Reg r) r' e = (if r = r' then e else Reg r)" |
-    "subst (Exp f rs) r e = (Exp f (map (\<lambda>x. subst x r e) rs))" |
-    "subst e _ _ = e"
-
-datatype ('v,'r) bexp = Neg "('v,'r) bexp" | Exp\<^sub>B "'v list \<Rightarrow> bool" "('v,'r) exp list"
-
-text \<open>Evaluate an expression given a register state\<close>
-fun ev\<^sub>B :: "('r \<Rightarrow> 'v) \<Rightarrow> ('v,'r) bexp \<Rightarrow> bool"
-  where 
-    "ev\<^sub>B m (Neg e) = (\<not> (ev\<^sub>B m e))" |
-    "ev\<^sub>B m (Exp\<^sub>B f rs) = f (map (ev m) rs)"
-
-text \<open>The syntactic register dependencies of an expression\<close>
-fun deps\<^sub>B :: "('v,'r) bexp \<Rightarrow> 'r set"
-  where 
-    "deps\<^sub>B (Neg e) = deps\<^sub>B e" |
-    "deps\<^sub>B (Exp\<^sub>B _ rs) = \<Union>(deps ` set rs)"
-
-text \<open>The global dependencies of an expression\<close>
-fun glbs\<^sub>B :: "('v,'r) bexp \<Rightarrow> 'v set"
-  where
-    "glbs\<^sub>B (Neg e) = glbs\<^sub>B e" |
-    "glbs\<^sub>B (Exp\<^sub>B _ rs) = \<Union>(glbs ` set rs)"
-
-text \<open>Substitute a register for an expression\<close>
-fun subst\<^sub>B :: "('v,'r) bexp \<Rightarrow> 'r \<Rightarrow> ('v,'r) exp \<Rightarrow> ('v,'r) bexp"
-  where
-    "subst\<^sub>B (Neg b) r e = Neg (subst\<^sub>B b r e)" |
-    "subst\<^sub>B (Exp\<^sub>B f rs) r e = (Exp\<^sub>B f (map (\<lambda>x. subst x r e) rs))"
-
-section \<open>Sub-operations\<close>
-
-text \<open>
-To model the possible reordering behaviour seen in ARMv8, it is necessary
-to model each operation as a series of sub-operations.
-For example a load would consist of an operation that first determines the memory address
-to access, followed by the memory access, followed by a store to a register.
-\<close>
-datatype ('v,'r) subop =
-    load 'v "('v,'r) exp"
-  | store 'v "('v,'r) exp"
-  | cas\<^sub>T 'v "('v,'r) exp" "('v,'r) exp"
-  | cas\<^sub>F 'v "('v,'r) exp" "('v,'r) exp"
-  | op 'r "('v,'r) exp"
-  | cmp "('v,'r) bexp"
-  | fence
-  | cfence
-  | stfence
-  | nop
-
-text \<open>Common Sub-Instructions\<close>
-abbreviation assign
-  where "assign r v \<equiv> op r (Exp (\<lambda>x. v) [])"
-
-abbreviation ncmp
-  where "ncmp b \<equiv> cmp (Neg b)"
-
-abbreviation eq
-  where "eq e\<^sub>1 e\<^sub>2 \<equiv> cmp (Exp\<^sub>B (\<lambda>x. x ! 0 = x ! 1) [e\<^sub>1,e\<^sub>2])"
-
-text \<open>Sub-operation execution behaviour\<close>
-fun beh\<^sub>i :: "('v,'r) subop \<Rightarrow> ('v,'r,'a) tstate rel"
-  where
-    "beh\<^sub>i (store a e) = {(m,m'). m' = m (a :=\<^sub>s ev (rg m) e)}" |
-    "beh\<^sub>i (load a e) = {(m,m'). m' = m \<and> st m a = ev (rg m) e}" |
-    "beh\<^sub>i (cas\<^sub>T a e\<^sub>1 e\<^sub>2) = {(m,m'). m' = m (a :=\<^sub>s ev (rg m) e\<^sub>2) \<and> st m a = ev (rg m) e\<^sub>1}" |
-    "beh\<^sub>i (cas\<^sub>F a e\<^sub>1 e\<^sub>2) = {(m,m'). m' = m \<and> st m a \<noteq> ev (rg m) e\<^sub>1}" |
-    "beh\<^sub>i (op r e) = {(m,m'). m' = m (r :=\<^sub>r ev (rg m) e)}" |
-    "beh\<^sub>i (cmp b) = {(m,m'). m = m' \<and> ev\<^sub>B (rg m) b}" |
-    "beh\<^sub>i _ = Id"
-
-text \<open>Memory addresses written by a sub-operation\<close>
-fun wr\<^sub>s :: "('v,'r) subop \<Rightarrow> 'v set"
-  where 
-    "wr\<^sub>s (store y _) = {y}" |
-    "wr\<^sub>s (cas\<^sub>T y _ _) = {y}" |
-    "wr\<^sub>s _ = {}"
-
-text \<open>Memory addresses reads by a sub-operation\<close>
-fun rd\<^sub>s :: "('v,'r) subop \<Rightarrow> 'v set"
-  where 
-    "rd\<^sub>s (load y _) = {y}" |
-    "rd\<^sub>s (cas\<^sub>T y _ _) = {y}" |
-    "rd\<^sub>s (cas\<^sub>F y _ _) = {y}" |
-    "rd\<^sub>s _ = {}"
-
-text \<open>Memory addresses accessed by a sub-operation\<close>
-abbreviation mems
-  where "mems \<alpha> \<equiv> rd\<^sub>s \<alpha> \<union> wr\<^sub>s \<alpha>"
-
-text \<open>Registers written by a sub-operation\<close>
-fun wr\<^sub>r :: "('v,'r) subop \<Rightarrow> 'r set"
-  where 
-    "wr\<^sub>r (op r _) = {r}" |
-    "wr\<^sub>r _ = {}"
-
-text \<open>Registers read by a sub-operation\<close>
-fun rd\<^sub>r :: "('v,'r) subop \<Rightarrow> 'r set"
-  where
-    "rd\<^sub>r (op _ e) = deps e" |
-    "rd\<^sub>r (store _ e) = deps e" |
-    "rd\<^sub>r (load _ e) = deps e" |
-    "rd\<^sub>r (cas\<^sub>T _ e\<^sub>1 e\<^sub>2) = deps e\<^sub>1 \<union> deps e\<^sub>2" |
-    "rd\<^sub>r (cas\<^sub>F _ e\<^sub>1 e\<^sub>2) = deps e\<^sub>1 \<union> deps e\<^sub>2" |
-    "rd\<^sub>r (cmp b) = deps\<^sub>B b" |
-    "rd\<^sub>r _ = {}"
-
-text \<open>Tagged memory addresses an expression is dependent on\<close>
-fun tags :: "('v,'r) subop \<Rightarrow> 'v set"
-  where 
-    "tags (op _ e) = glbs e" |
-    "tags (store _ e) = glbs e" |
-    "tags (load _ e) = glbs e" |
-    "tags (cas\<^sub>T _ e\<^sub>1 e\<^sub>2) = glbs e\<^sub>1 \<union> glbs e\<^sub>2" |
-    "tags (cas\<^sub>F _ e\<^sub>1 e\<^sub>2) = glbs e\<^sub>1 \<union> glbs e\<^sub>2" |
-    "tags (cmp b) = glbs\<^sub>B b" |
-    "tags _ = {}"
 
 text \<open>Sub-Instruction Reordering\<close>
 text \<open>Only pattern match on first argument due to performance issues\<close>
 fun re\<^sub>i :: "('v,'r) subop \<Rightarrow> ('v,'r) subop \<Rightarrow> bool" 
   where
     "re\<^sub>i fence \<alpha> = False" |
-    "re\<^sub>i stfence \<alpha> = (wr\<^sub>s \<alpha> = {})" |
-    "re\<^sub>i (cmp b) \<alpha> = (wr\<^sub>s \<alpha> = {} \<and> \<alpha> \<noteq> cfence  \<and> rd\<^sub>r (cmp b) \<inter> wr\<^sub>r \<alpha> = {})" |
-    "re\<^sub>i cfence \<alpha> = (rd\<^sub>s \<alpha> = {})" |
-    "re\<^sub>i \<alpha> \<beta> = (\<alpha> \<noteq> fence \<and>
-                (\<alpha> = stfence \<longrightarrow> wr\<^sub>s \<beta> = {}) \<and>
-                mems \<alpha> \<inter> mems \<beta> = {} \<and> 
-                mems \<alpha> \<inter> tags \<beta> = {} \<and> 
-                wr\<^sub>r \<alpha> \<inter> wr\<^sub>r \<beta> = {} \<and> 
-                rd\<^sub>r \<alpha> \<inter> wr\<^sub>r \<beta> = {})"
-  
+    "re\<^sub>i stfence \<alpha> = (\<alpha> \<noteq> fence \<and> wr \<alpha> \<subseteq> locals)" |
+    "re\<^sub>i cfence \<alpha> = (\<alpha> \<noteq> fence \<and> rd \<alpha> \<subseteq> locals)" |
+    "re\<^sub>i (cmp b) \<alpha> = (wr \<alpha> \<subseteq> locals \<and> \<alpha> \<noteq> cfence \<and> \<alpha> \<noteq> fence \<and> rd (cmp b) \<inter> wr \<alpha> = {})" |
+    "re\<^sub>i \<alpha> \<beta> = (\<beta> \<noteq> fence \<and> (\<beta> = stfence \<longrightarrow> wr \<alpha> \<subseteq> locals) \<and> (\<beta> = cfence \<longrightarrow> \<not>(\<exists>b. \<alpha> = cmp b)) \<and>
+                (wr \<alpha> \<union> rd \<alpha>) \<inter> rd \<beta> \<subseteq> locals \<and> 
+                wr \<alpha> \<inter> wr \<beta> = {} \<and> 
+                rd \<alpha> \<inter> wr \<beta> = {})"
+
 text \<open>Sub-Instruction Forwarding\<close>
 fun fwd\<^sub>i :: "('v,'r) subop \<Rightarrow> ('v,'r) subop \<Rightarrow> ('v,'r) subop" 
   where
-    "fwd\<^sub>i (load v\<^sub>a r\<^sub>a) (store v\<^sub>b r\<^sub>b) = (if v\<^sub>a = v\<^sub>b then eq r\<^sub>a r\<^sub>b else load v\<^sub>a r\<^sub>a)" |
-    "fwd\<^sub>i (load v\<^sub>a r\<^sub>a) (cas\<^sub>T v\<^sub>b _ e\<^sub>2) = (if v\<^sub>a = v\<^sub>b then eq r\<^sub>a e\<^sub>2 else load v\<^sub>a r\<^sub>a)" |
-    "fwd\<^sub>i (store v\<^sub>a e) (op r e') = (store v\<^sub>a (subst e r e'))" |
-    "fwd\<^sub>i (load v\<^sub>a e) (op r e') = (load v\<^sub>a (subst e r e'))" |
-    "fwd\<^sub>i (cmp b) (op r e) = (cmp (subst\<^sub>B b r e))" |
-    "fwd\<^sub>i (op r e) (op r' e') = (op r (subst e r' e'))" |
-    "fwd\<^sub>i (cas\<^sub>T v\<^sub>a e\<^sub>1 e\<^sub>2) (op r e) = (cas\<^sub>T v\<^sub>a (subst e\<^sub>1 r e) (subst e\<^sub>2 r e))" |
-    "fwd\<^sub>i (cas\<^sub>F v\<^sub>a e\<^sub>1 e\<^sub>2) (op r e) = (cas\<^sub>F v\<^sub>a (subst e\<^sub>1 r e) (subst e\<^sub>2 r e))" |
+    "fwd\<^sub>i \<alpha> (cstore b g e) = subst\<^sub>g \<alpha> g e" |
+    "fwd\<^sub>i \<alpha> (cas\<^sub>T g _ e) = subst\<^sub>g \<alpha> g e" |
+    "fwd\<^sub>i \<alpha> (op r e) = subst\<^sub>r \<alpha> r e" |
     "fwd\<^sub>i \<alpha> _ = \<alpha>"
 
-lemma [simp]:
-  "ev m (subst e r f) = ev (m(r := (ev m f))) e"
-proof (induct e)
-  case (Exp fn rs)
-  hence [simp]: "map (ev m \<circ> (\<lambda>x. subst x r f)) rs = map (ev (\<lambda>a. if a = r then ev m f else m a)) rs"
-    by auto
-  show ?case by simp
-qed auto
-
-lemma [simp]:
-  "ev\<^sub>B m (subst\<^sub>B b r e) = ev\<^sub>B (m(r := (ev m e))) b"
-proof (induct b)
-  case (Exp\<^sub>B fn rs)
-  have [simp]: "map (ev m \<circ> (\<lambda>x. subst x r e)) rs = map (ev (\<lambda>a. if a = r then ev m e else m a)) rs"
-    by (auto simp: fun_upd_def)     
-  show ?case by simp
-qed simp
-
-lemma ev_nop [simp]:
-  "r \<notin> deps e \<Longrightarrow> ev (m(r := f)) e = ev m e"
-proof (induct e)
-  case (Exp fn rs)
-  hence [simp]: "map (ev (\<lambda>a. if a = r then f else m a)) rs = (map (ev m) rs)" by auto
-  show ?case by simp
-qed auto
-
-lemma ev\<^sub>B_nop [simp]:
-  "r \<notin> deps\<^sub>B b \<Longrightarrow> ev\<^sub>B (m(r := f)) b = ev\<^sub>B m b"
-proof (induct b)
-  case (Exp\<^sub>B fn rs)
-  hence [simp]: "map (ev (\<lambda>a. if a = r then f else m a)) rs = map (ev m) rs"
-    using ev_nop[of r _ m f] by (auto simp: fun_upd_def) 
-  show ?case by simp
-qed simp
-
-definition comp (infix "\<Otimes>" 60)
+definition comp (infixr "\<Otimes>" 60)
   where "comp a b \<equiv> {(m,m'). \<exists>m''. (m,m'') \<in> a \<and> (m'',m') \<in> b}"
+
+lemma [simp]:
+  "(Reg x \<notin> Reg ` e) = (x \<notin> e)"
+  by blast
 
 lemma re_consistent:
   "re\<^sub>i \<alpha> (fwd\<^sub>i \<beta> \<alpha>) \<Longrightarrow> beh\<^sub>i \<alpha> \<Otimes> beh\<^sub>i \<beta> \<supseteq> beh\<^sub>i (fwd\<^sub>i \<beta> \<alpha>) \<Otimes> beh\<^sub>i \<alpha>" 
-  by (cases \<alpha>; cases \<beta>; auto simp add: comp_def st_upd_def rg_upd_def intro!: fun_upd_twist equality)
- 
+  by (cases \<alpha>; cases \<beta>; clarsimp simp add: comp_def fun_upd_twist split: if_splits)
+
 section \<open>Auxiliary State Updates\<close>
 
 text \<open>
@@ -241,21 +47,21 @@ This auxiliary state cannot influence real execution behaviour by definition.
 \<close>
 type_synonym ('v,'r,'a) auxop = "('v,'r) subop \<times> ('v,'r,'a) auxfn"
 
-fun beh\<^sub>a :: "('v,'r,'a) auxop \<Rightarrow> ('v,'r,'a) tstate rel"
+fun beh\<^sub>a :: "('v,'r,'a) auxop \<Rightarrow> ('v,'r,'a) state rel"
   where "beh\<^sub>a (\<alpha>,f) = beh\<^sub>i \<alpha> O {(m,m'). m' = m(aux: f)}"
 
 fun re\<^sub>a :: "('v,'r,'a) auxop \<Rightarrow> ('v,'r,'a) auxop \<Rightarrow> bool" 
   where "re\<^sub>a (\<alpha>,f) (\<beta>,f') = re\<^sub>i \<alpha> \<beta>"
 
 fun fwd\<^sub>a :: "('v,'r,'a) auxop \<Rightarrow> ('v,'r,'a) auxop \<Rightarrow> ('v,'r,'a) auxop" 
-  where "fwd\<^sub>a (\<alpha>,f) (\<beta>,f') = (fwd\<^sub>i \<alpha> \<beta>,f)"
+  where "fwd\<^sub>a (\<alpha>,f) \<beta> = (fwd\<^sub>i \<alpha> (fst \<beta>),f)"
 
 section \<open>Sub-Instruction Specification Language\<close>
 
 text \<open>
 To instantiate the abstract theory, we must couple each sub-operation with its precondition
 and behaviour in a tuple\<close>
-type_synonym ('v,'r,'a) subbasic = "(('v,'r,'a) auxop, ('v,'r,'a) tstate) basic"
+type_synonym ('v,'r,'a) subbasic = "(('v,'r,'a) auxop, ('v,'r,'a) state) basic"
 
 text \<open>Duplicate forwarding and reordering behaviour of underlying instruction\<close>
 fun fwd\<^sub>s :: "('v,'r,'a) subbasic \<Rightarrow> ('v,'r,'a) auxop \<Rightarrow> ('v,'r,'a) subbasic" 
@@ -264,12 +70,12 @@ fun fwd\<^sub>s :: "('v,'r,'a) subbasic \<Rightarrow> ('v,'r,'a) auxop \<Rightar
 text \<open>Lift an operation with specification\<close>
 definition liftg :: "('v,'r,'a) pred \<Rightarrow> ('v,'r) subop \<Rightarrow> ('v,'r,'a) auxfn \<Rightarrow> ('v,'r,'a) subbasic" 
   ("\<lfloor>_,_,_\<rfloor>" 100)
-  where "liftg v \<alpha> f \<equiv> ((\<alpha>,f), Collect v, beh\<^sub>a (\<alpha>,f))"
+  where "liftg v \<alpha> f \<equiv> ((\<alpha>,f), v, beh\<^sub>a (\<alpha>,f))"
 
 text \<open>Lift an operation without specification\<close>
 definition liftl :: "('v,'r) subop \<Rightarrow> ('v,'r,'a) subbasic" 
   ("\<lfloor>_\<rfloor>" 100)
-  where "liftl \<alpha> \<equiv> ((\<alpha>,tstate_rec.more), UNIV, beh\<^sub>a (\<alpha>,tstate_rec.more))"
+  where "liftl \<alpha> \<equiv> ((\<alpha>,aux), UNIV, beh\<^sub>a (\<alpha>,aux))"
 
 section \<open>ARMv8 Language Definition\<close>
 
@@ -287,9 +93,5 @@ datatype ('v,'r,'a) com_armv8 =
   | CAS "('v,'r,'a) pred" 'r 'r 'r 'r 'v 'v "('v,'r,'a) auxfn"
   | Seq "('v,'r,'a) com_armv8" "('v,'r,'a) com_armv8"
   | If "('v,'r) bexp" "('v,'r,'a) com_armv8" "('v,'r,'a) com_armv8"
-  | While "('v,'r) bexp" "('v,'r,'a) pred" "('v,'r,'a) com_armv8"
-  | DoWhile "('v,'r,'a) pred" "('v,'r,'a) com_armv8" "('v,'r) bexp"
-  | Test "('v,'r,'a) pred"
-  | Assert "('v,'r,'a) pred"
 
 end
