ARMv8/ARMv8_Rules.thy
@@ -4,32 +4,37 @@ begin
 
 section \<open>Wellformedness\<close>
 
-text \<open>
-Abstract theory is in terms of sets of states, where as the WP reasoning uses functions.
-This lifting converts to the abstract.
-\<close>
-abbreviation lift_encoding ("\<langle>_\<rangle>" 1000) 
-  where "lift_encoding \<equiv> Collect"
+definition stabilize
+  where "stabilize R P \<equiv> {m. \<forall>m'. (glb m,glb m') \<in> R \<longrightarrow> rg m = rg m' \<longrightarrow> m' \<in> P}"
 
-text \<open>Lift an invariant to a relation\<close>
-definition inv :: "(('v,'a) gstate \<Rightarrow> bool) \<Rightarrow> ('v,'a) grel"
-  where "inv I \<equiv> \<lambda>(m,m'). I m \<longrightarrow> I m'"
+definition reflexive
+  where "reflexive R \<equiv> \<forall>m. (m,m) \<in> R"
 
-text \<open>Convert a global predicate into a thread local predicate by ignoring the local state\<close>
-definition all\<^sub>t :: "(('v,'a) gstate \<Rightarrow> bool) \<Rightarrow> ('v,'r,'a) pred"
-  where "all\<^sub>t I \<equiv> \<lambda>m. I (glb m)"
+definition transitive
+  where "transitive R \<equiv> \<forall>m m' m''. (m,m') \<in> R \<longrightarrow> (m',m'') \<in> R \<longrightarrow> (m,m'') \<in> R"
 
-text \<open>Lift a relational predicate with no constraint on thread state\<close>
-definition step :: "('v,'a) grel \<Rightarrow> ('v,'r,'a) trel"
-  where "step R \<equiv> \<lambda>(m,m'). R (glb m, glb m')"
+definition assert
+  where "assert b \<equiv> {m. b}"
 
 text \<open>Lift a relational predicate and assume it preserves the thread state\<close>
 definition step\<^sub>t :: "('v,'a) grel \<Rightarrow> ('v,'r,'a) trel"
-  where "step\<^sub>t R \<equiv> \<lambda>(m,m'). R (glb m, glb m') \<and> rg m = rg m'"
+  where "step\<^sub>t R \<equiv> {(m,m'). (glb m, glb m') \<in> R \<and> rg m = rg m'}"
+
+text \<open>Lift a relational predicate\<close>
+definition step :: "('v,'a) grel \<Rightarrow> ('v,'r,'a) trel"
+  where "step R \<equiv> {(m,m'). (glb m, glb m') \<in> R}"
 
 text \<open>Define stability in terms of a relational predicate that preserves the thread state\<close>
 abbreviation stable\<^sub>t
-  where "stable\<^sub>t R P \<equiv> stable \<langle>step\<^sub>t R\<rangle> \<langle>P\<rangle>"
+  where "stable\<^sub>t R P \<equiv> stable (step\<^sub>t R) P"
+
+text \<open>Lift an invariant to a relation\<close>
+definition inv :: "(('v,'a) gstate set) \<Rightarrow> ('v,'a) grel"
+  where "inv I \<equiv> {(m,m'). m \<in> I \<longrightarrow> m' \<in> I}"
+
+text \<open>Convert a global predicate into a thread local predicate by ignoring the local state\<close>
+definition all\<^sub>t :: "(('v,'a) gstate set) \<Rightarrow> ('v,'r,'a) pred"
+  where "all\<^sub>t I \<equiv> {m. (glb m) \<in> I}"
 
 text \<open>Couple all wellformedness conditions into a single definition\<close>
 abbreviation wellformed :: "('v,'a) grel \<Rightarrow> ('v,'a) grel \<Rightarrow> bool"
@@ -42,58 +47,57 @@ lemma stabilize_stable [intro]:
   unfolding stable_def step\<^sub>t_def
 proof (clarsimp)
   fix m m'
-  assume a: "stabilize R Q m" "R (glb m, glb m')" "rg m = rg m'"
-  have "\<forall>g''. R (glb m',g'') \<longrightarrow> R (glb m,g'')"
+  assume a: "m \<in> stabilize R Q" "(glb m, glb m') \<in> R" "rg m = rg m'"
+  have "\<forall>g''. (glb m',g'') \<in> R \<longrightarrow> (glb m,g'') \<in> R"
     using assms a(2) unfolding transitive_def by blast
-  thus "stabilize R Q m'" using a(1,3) by (auto simp: stabilize_def set_glb_def)
+  thus "m' \<in> stabilize R Q" using a(1,3) by (auto simp: stabilize_def)
 qed
 
 text \<open>The conjunction of two stable predicates is stable\<close>
 lemma stable\<^sub>t_conj [intro]:
   assumes "stable\<^sub>t R P" "stable\<^sub>t R Q"
-  shows "stable\<^sub>t R (P \<and>\<^sub>p Q)"
-  using assms by (auto simp: stable_def pred_defs)
+  shows "stable\<^sub>t R (P \<inter> Q)"
+  using assms by (auto simp: stable_def)
 
 text \<open>Elimination rule to ignore the stabilization process\<close>
 lemma stabilizeE:
-  assumes "stabilize R P m"
-  assumes "wellformed R G"
-  obtains "P m"
+  assumes "m \<in> stabilize R P"
+  assumes "reflexive R"
+  obtains "m \<in> P"
 proof -
-  have "\<forall>g. R (glb m, g) \<longrightarrow> P (set_glb m g)" "R (glb m, glb m)"
+  have "\<forall>g. (glb m, glb g) \<in> R \<longrightarrow> rg m = rg g \<longrightarrow> g \<in> P" "(glb m, glb m) \<in>  R"
     using assms by (auto simp: reflexive_def stabilize_def)
   thus ?thesis using that by auto
 qed
 
 text \<open>Stabilization preserves entailment\<close>
-lemma stabilize_entail [intro!]:
-  assumes "wellformed R G"
-  assumes "P \<turnstile>\<^sub>p Q"
-  shows "stabilize R P \<turnstile>\<^sub>p Q"
-  using assms by (auto simp: pred_defs stabilize_def)
+lemma stabilize_entail :
+  assumes "m \<in> stabilize R P" 
+  assumes "reflexive R"
+  assumes "P \<subseteq> Q"
+  shows "m \<in> stabilize R Q"
+  using assms by (auto simp: stabilize_def)
 
 section \<open>Predicate Transformations\<close>
-
-named_theorems wp_defs
 
 text \<open>Transform a predicate based on an sub-operation\<close>
 fun wp\<^sub>i :: "('v,'r) subop \<Rightarrow> ('v,'r,'a) trans" 
   where 
-    "wp\<^sub>i (load v e) Q = (\<lambda>m. st m v = ev (rg m) e \<longrightarrow> Q m)" | 
-    "wp\<^sub>i (store v e) Q = (\<lambda>m. Q (m(v :=\<^sub>s ev (rg m) e)))" | 
-    "wp\<^sub>i (op r e) Q = (\<lambda>m. Q (m (r :=\<^sub>r ev (rg m) e)))" |
-    "wp\<^sub>i (cmp b) Q = (\<lambda>m. ev\<^sub>B (rg m) b \<longrightarrow> Q m)" | 
-    "wp\<^sub>i (cas\<^sub>T v e\<^sub>1 e\<^sub>2) Q = (\<lambda>m. st m v = ev (rg m) e\<^sub>1 \<longrightarrow> Q (m(v :=\<^sub>s ev (rg m) e\<^sub>2)))" | 
-    "wp\<^sub>i (cas\<^sub>F v e\<^sub>1 e\<^sub>2) Q = (\<lambda>m. st m v \<noteq> ev (rg m) e\<^sub>1 \<longrightarrow> Q m)" | 
+    "wp\<^sub>i (load v e) Q = {m. st m (Glb v) = ev\<^sub>E (rg m) e \<longrightarrow> m \<in> Q}" | 
+    "wp\<^sub>i (cstore b v e) Q = {m. ev\<^sub>B (rg m) b \<longrightarrow> (m(Glb v :=\<^sub>s ev\<^sub>E (rg m) e)) \<in> Q}" | 
+    "wp\<^sub>i (op r e) Q = {m. m(Reg r :=\<^sub>s ev\<^sub>E (rg m) e) \<in> Q}" |
+    "wp\<^sub>i (cmp b) Q = {m. ev\<^sub>B (rg m) b \<longrightarrow> m \<in> Q}" | 
+    "wp\<^sub>i (cas\<^sub>T v e\<^sub>1 e\<^sub>2) Q = {m. st m (Glb v) = ev\<^sub>E (rg m) e\<^sub>1 \<longrightarrow> m(Glb v :=\<^sub>s ev\<^sub>E (rg m) e\<^sub>2) \<in> Q}" | 
+    "wp\<^sub>i (cas\<^sub>F v e\<^sub>1) Q = {m. st m (Glb v) \<noteq> ev\<^sub>E (rg m) e\<^sub>1 \<longrightarrow> m \<in> Q}" | 
     "wp\<^sub>i _ Q = Q"
 
 text \<open>Transform a predicate based on an auxiliary state update\<close>
 fun wp\<^sub>a :: "('v,'r,'a) auxfn \<Rightarrow> ('v,'r,'a) trans"
-  where "wp\<^sub>a a Q = (\<lambda>m. Q (m(aux: a)))"
+  where "wp\<^sub>a a Q = {m. (m(aux: a)) \<in> Q}"
 
 datatype ('v,'r,'a) insts =
   ld "('v,'r,'a) pred" "('v,'r) exp" 'r "('v,'r,'a) auxfn"
-  | sr "('v,'r,'a) pred" "('v,'r) exp" 'r "('v,'r,'a) auxfn"
+  | sr "('v,'r,'a) pred" "('v,'r) bexp" "('v,'r) exp" 'r "('v,'r,'a) auxfn"
   | ir 'r "('v,'r) exp" 
   | cm "('v,'r) bexp"
   | ncm "('v,'r) bexp"
@@ -101,8 +105,8 @@ datatype ('v,'r,'a) insts =
 
 fun wpre :: "('v,'r,'a) insts \<Rightarrow> ('v,'r,'a) trans"
   where
-    "wpre (ld v r\<^sub>a r a) Q = ((\<lambda>m. v m \<and> Q (m (r :=\<^sub>r st m (ev (rg m) r\<^sub>a), aux: a))))" |
-    "wpre (sr v r\<^sub>a r a) Q = ( (\<lambda>m. v m \<and> Q (m (ev (rg m) r\<^sub>a :=\<^sub>s rg m r, aux: a))))" |
+    "wpre (ld v r\<^sub>a r a) Q = {m. m \<in> v \<and> (m (Reg r :=\<^sub>s st m (Glb (ev\<^sub>E (rg m) r\<^sub>a)), aux: a)) \<in> Q}" |
+    "wpre (sr v b r\<^sub>a r a) Q = {m. m \<in> v \<and> (ev\<^sub>B (rg m) b \<longrightarrow> (m (Glb (ev\<^sub>E (rg m) r\<^sub>a) :=\<^sub>s rg m r, aux: a)) \<in> Q)}" |
     "wpre (ir r e) Q = wp\<^sub>i (op r e) Q" |
     "wpre (cm b) Q = wp\<^sub>i (cmp b) Q" |
     "wpre (ncm b) Q = wp\<^sub>i (ncmp b) Q" |
@@ -111,19 +115,16 @@ fun wpre :: "('v,'r,'a) insts \<Rightarrow> ('v,'r,'a) trans"
 text \<open>Transform a predicate based on a successful CAS instruction\<close>
 definition wp_CAS\<^sub>T :: "'r \<Rightarrow> 'r \<Rightarrow> 'r \<Rightarrow> 'r \<Rightarrow> 'v \<Rightarrow> 'v \<Rightarrow> ('v,'r,'a) auxfn \<Rightarrow> ('v,'r,'a) trans"
   where "wp_CAS\<^sub>T r\<^sub>a r\<^sub>1 r\<^sub>2 r T F a Q \<equiv> 
-    \<lambda>m. st m (rg m r\<^sub>a) = rg m r\<^sub>1 \<longrightarrow> Q (m(rg m r\<^sub>a :=\<^sub>s rg m r\<^sub>2, r :=\<^sub>r T, aux: a))"
-declare wp_CAS\<^sub>T_def [wp_defs]
+    {m. st m (Glb (rg m r\<^sub>a)) = st m (Reg r\<^sub>1) \<longrightarrow> (m(Glb (rg m r\<^sub>a) :=\<^sub>s rg m r\<^sub>2, Reg r :=\<^sub>s T, aux: a)) \<in> Q}"
 
 text \<open>Transform a predicate based on a failed CAS instruction\<close>
 definition wp_CAS\<^sub>F :: "'r \<Rightarrow> 'r \<Rightarrow> 'r \<Rightarrow> 'r \<Rightarrow> 'v \<Rightarrow> 'v \<Rightarrow> ('v,'r,'a) auxfn \<Rightarrow> ('v,'r,'a) trans"
   where "wp_CAS\<^sub>F r\<^sub>a r\<^sub>1 r\<^sub>2 r T F a Q \<equiv> 
-    \<lambda>m. st m (rg m r\<^sub>a) \<noteq> rg m r\<^sub>1 \<longrightarrow> Q (m(r :=\<^sub>r F, aux: a))"
-declare wp_CAS\<^sub>F_def [wp_defs]
+    {m. st m (Glb (rg m r\<^sub>a)) \<noteq> st m (Reg r\<^sub>1) \<longrightarrow> (m(Reg r :=\<^sub>s F, aux: a)) \<in> Q}"
 
 text \<open>Transform a predicate based on a CAS instruction\<close>
 definition wp_CAS :: "'r \<Rightarrow> 'r \<Rightarrow> 'r \<Rightarrow> 'r \<Rightarrow> 'v \<Rightarrow> 'v \<Rightarrow> ('v,'r,'a) auxfn \<Rightarrow> ('v,'r,'a) trans"
-  where "wp_CAS r\<^sub>a r\<^sub>1 r\<^sub>2 r T F a Q \<equiv> wp_CAS\<^sub>T r\<^sub>a r\<^sub>1 r\<^sub>2 r T F a Q \<and>\<^sub>p wp_CAS\<^sub>F r\<^sub>a r\<^sub>1 r\<^sub>2 r T F a Q"
-declare wp_CAS_def [wp_defs]
+  where "wp_CAS r\<^sub>a r\<^sub>1 r\<^sub>2 r T F a Q \<equiv> wp_CAS\<^sub>T r\<^sub>a r\<^sub>1 r\<^sub>2 r T F a Q \<inter> wp_CAS\<^sub>F r\<^sub>a r\<^sub>1 r\<^sub>2 r T F a Q"
 
 text \<open>Transform a predicate based on a program c within an environment R\<close>
 fun wp :: "('v,'a) grel \<Rightarrow> ('v,'r,'a) com_armv8 \<Rightarrow> ('v,'r,'a) trans"
@@ -131,92 +132,71 @@ fun wp :: "('v,'a) grel \<Rightarrow> ('v,'r,'a) com_armv8 \<Rightarrow> ('v,'r,
     "wp R Skip Q = Q" |
     "wp R Fence Q = Q" |
     "wp R (Load v r\<^sub>a r a) Q = stabilize R (wpre (ld v r\<^sub>a r a) Q)" |
-    "wp R (Store v r\<^sub>a r a) Q = stabilize R (wpre (sr v r\<^sub>a r a) Q)" |
+    "wp R (Store v r\<^sub>a r a) Q = stabilize R (wpre (sr v True\<^sub>B r\<^sub>a r a) Q)" |
     "wp R (Op r e) Q = wpre (ir r e) Q" |
-    "wp R (Test p) Q = stabilize R (p \<longrightarrow>\<^sub>p Q)" |
-    "wp R (Assert p) Q = (stabilize R p \<and>\<^sub>p Q)" |
-    "wp R (CAS v r\<^sub>a r\<^sub>1 r\<^sub>2 r T F a) Q = stabilize R (v \<and>\<^sub>p wp_CAS r\<^sub>a r\<^sub>1 r\<^sub>2 r T F a Q)" |
+    "wp R (CAS v r\<^sub>a r\<^sub>1 r\<^sub>2 r T F a) Q = stabilize R (v \<inter> wp_CAS r\<^sub>a r\<^sub>1 r\<^sub>2 r T F a Q)" |
     "wp R (Seq c\<^sub>1 c\<^sub>2) Q = wp R c\<^sub>1 (wp R c\<^sub>2 Q)" |
-    "wp R (If b c\<^sub>1 c\<^sub>2) Q = (wpre (cm b) (wp R c\<^sub>1 Q) \<and>\<^sub>p wpre (ncm b) (wp R c\<^sub>2 Q))" |
-    "wp R (While b I c) Q = 
-      (stabilize R I \<and>\<^sub>p assert (I \<turnstile>\<^sub>p wp\<^sub>i (cmp b) (wp R c (stabilize R I)) \<and>\<^sub>p wp\<^sub>i (ncmp b) Q))" |
-    "wp R (DoWhile I c b) Q = 
-      (stabilize R I \<and>\<^sub>p assert (I \<turnstile>\<^sub>p wp R c (wp\<^sub>i (cmp b) (stabilize R I) \<and>\<^sub>p wp\<^sub>i (ncmp b) Q)))"
+    "wp R (If b c\<^sub>1 c\<^sub>2) Q = (wpre (cm b) (wp R c\<^sub>1 Q) \<inter> wpre (ncm b) (wp R c\<^sub>2 Q))"
 
 text \<open>Convert a predicate transformer into a relational predicate transformer\<close>
 definition wp\<^sub>r :: "('v,'r,'a) trans \<Rightarrow> ('v,'r,'a) rtrans"
-  where "wp\<^sub>r f G \<equiv> \<lambda>(m,m'). f (\<lambda>m'. G (m,m')) m'"
-declare wp\<^sub>r_def [wp_defs]
-
-text \<open>Conditions under which a relational predicate is reflexive\<close>
-definition refl :: "('v,'r,'a) trel \<Rightarrow> ('v,'r,'a) pred"
-  where "refl G \<equiv> \<lambda>m. G (m,m)"
-declare refl_def [wp_defs]
+  where "wp\<^sub>r f G \<equiv> {(m,m'). m' \<in> f {m'. (m,m') \<in> G}}"
 
 subsection \<open>Guarantee Checks\<close>
 
 text \<open>Convert a predicate transformer into a guarantee check\<close>
 abbreviation guar
-  where "guar f G \<equiv> refl (wp\<^sub>r f G)"
+  where "guar f G \<equiv> {m. (m,m) \<in> (wp\<^sub>r f G)}"
 
 text \<open>Ensure all global operations in a thread conform to its guarantee\<close>
 fun guar\<^sub>c
   where 
-    "guar\<^sub>c (Load v r\<^sub>a r a) G = (v \<turnstile>\<^sub>p guar (wpre (ld True\<^sub>p r\<^sub>a r a)) (step G))" |
-    "guar\<^sub>c (Store v r\<^sub>a r a) G = (v \<turnstile>\<^sub>p guar (wpre (sr True\<^sub>p r\<^sub>a r a)) (step G))" |
-    "guar\<^sub>c (CAS v r\<^sub>a r\<^sub>1 r\<^sub>2 r T F a) G = (v \<turnstile>\<^sub>p guar (wp_CAS r\<^sub>a r\<^sub>1 r\<^sub>2 r T F a) (step G))" |
+    "guar\<^sub>c (Load v r\<^sub>a r a) G = (v \<subseteq> guar (wpre (ld UNIV r\<^sub>a r a)) (step G))" |
+    "guar\<^sub>c (Store v r\<^sub>a r a) G = (v \<subseteq> guar (wpre (sr UNIV True\<^sub>B r\<^sub>a r a)) (step G))" |
+    "guar\<^sub>c (CAS v r\<^sub>a r\<^sub>1 r\<^sub>2 r T F a) G = (v \<subseteq> guar (wp_CAS r\<^sub>a r\<^sub>1 r\<^sub>2 r T F a) (step G))" |
     "guar\<^sub>c (Seq c\<^sub>1 c\<^sub>2) G = (guar\<^sub>c c\<^sub>1 G \<and> guar\<^sub>c c\<^sub>2 G)" |
     "guar\<^sub>c (If b c\<^sub>1 c\<^sub>2) G = (guar\<^sub>c c\<^sub>1 G \<and> guar\<^sub>c c\<^sub>2 G)" |
-    "guar\<^sub>c (While b I c) G = (guar\<^sub>c c G)" |
-    "guar\<^sub>c (DoWhile I c b) G = (guar\<^sub>c c G)" |
     "guar\<^sub>c _ _ = True"
 
 section \<open>Locale Interpretation\<close>
 
 text \<open>Convert the ARMv8 language into the abstract language expected by the underlying logic\<close> 
-fun lift\<^sub>c :: "('v,'r,'a) com_armv8 \<Rightarrow> (('v,'r,'a) auxop, ('v,'r,'a) tstate) com"
+fun lift\<^sub>c :: "('v,'r,'a) com_armv8 \<Rightarrow> (('v,'r,'a) auxop, ('v,'r,'a) state) com"
   where
     "lift\<^sub>c Skip = com.Nil" |
     "lift\<^sub>c Fence = Basic (\<lfloor>fence\<rfloor>)" |
     "lift\<^sub>c (Op r e) = Basic (\<lfloor>op r e\<rfloor>)" |
     "lift\<^sub>c (Load c r\<^sub>a r a) = \<Sqinter> {[
-      \<lfloor>eq ( r\<^sub>a) (Val v\<^sub>a)\<rfloor>, 
-      \<lfloor>(\<lambda>m. ev (rg m) r\<^sub>a = v\<^sub>a) \<and>\<^sub>p c,load v\<^sub>a (Val v), (\<lambda>m. a (m(r :=\<^sub>r v)))\<rfloor>, 
-      \<lfloor>op r (Glb v v\<^sub>a)\<rfloor>] |v v\<^sub>a. True}" |
+      \<lfloor>eq r\<^sub>a (Val v\<^sub>a)\<rfloor>, 
+      \<lfloor>{m. ev\<^sub>E (rg m) r\<^sub>a = v\<^sub>a} \<inter> c,load v\<^sub>a (Val v), (\<lambda>m. a (m(Reg r :=\<^sub>s v)))\<rfloor>, 
+      \<lfloor>op r (Val v)\<rfloor>] |v v\<^sub>a. True}" |
     "lift\<^sub>c (Store c r\<^sub>a r a) = \<Sqinter> {[
-      \<lfloor>eq ( r\<^sub>a) (Val v\<^sub>a)\<rfloor>, 
-      \<lfloor>(\<lambda>m. ev (rg m) r\<^sub>a = v\<^sub>a) \<and>\<^sub>p c,store v\<^sub>a (Reg r), a\<rfloor>] |v\<^sub>a. True}" |
+      \<lfloor>eq r\<^sub>a (Val v\<^sub>a)\<rfloor>, 
+      \<lfloor>{m. ev\<^sub>E (rg m) r\<^sub>a = v\<^sub>a} \<inter> c,cstore True\<^sub>B v\<^sub>a (Var r), a\<rfloor>] |v\<^sub>a. True}" |
     "lift\<^sub>c (CAS c r\<^sub>a r\<^sub>1 r\<^sub>2 r T F a) = (Choice
       (\<Sqinter> {[
-        \<lfloor>eq (Reg r\<^sub>a) (Val v\<^sub>a)\<rfloor>, 
-        \<lfloor>(\<lambda>m. rg m r\<^sub>a = v\<^sub>a) \<and>\<^sub>p c,cas\<^sub>T v\<^sub>a (Reg r\<^sub>1) (Reg r\<^sub>2),(\<lambda>m. a (m(r :=\<^sub>r T)))\<rfloor>, 
-        \<lfloor>op r (Glb T v\<^sub>a)\<rfloor>] |v\<^sub>a. True})
+        \<lfloor>eq (Var r\<^sub>a) (Val v\<^sub>a)\<rfloor>, 
+        \<lfloor>{m. rg m r\<^sub>a = v\<^sub>a} \<inter> c,cas\<^sub>T v\<^sub>a (Var r\<^sub>1) (Var r\<^sub>2),(\<lambda>m. a (m(Reg r :=\<^sub>s T)))\<rfloor>, 
+        \<lfloor>op r (Val T)\<rfloor>] |v\<^sub>a. True})
       (\<Sqinter> {[
-        \<lfloor>eq (Reg r\<^sub>a) (Val v\<^sub>a)\<rfloor>, 
-        \<lfloor>(\<lambda>m. rg m r\<^sub>a = v\<^sub>a) \<and>\<^sub>p c,cas\<^sub>F v\<^sub>a (Reg r\<^sub>1) (Reg r\<^sub>2),(\<lambda>m. a (m(r :=\<^sub>r F)))\<rfloor>, 
-        \<lfloor>op r (Glb F v\<^sub>a)\<rfloor>] |v\<^sub>a. True}))" |
+        \<lfloor>eq (Var r\<^sub>a) (Val v\<^sub>a)\<rfloor>, 
+        \<lfloor>{m. rg m r\<^sub>a = v\<^sub>a} \<inter> c,cas\<^sub>F v\<^sub>a (Var r\<^sub>1),(\<lambda>m. a (m(Reg r :=\<^sub>s F)))\<rfloor>, 
+        \<lfloor>op r (Val F)\<rfloor>] |v\<^sub>a. True}))" |
     "lift\<^sub>c (Seq c\<^sub>1 c\<^sub>2) = (lift\<^sub>c c\<^sub>1 ;; lift\<^sub>c c\<^sub>2)" |
     "lift\<^sub>c (If b c\<^sub>1 c\<^sub>2) = (Choice 
       (com.Seq (Basic (\<lfloor>cmp b\<rfloor>)) (lift\<^sub>c c\<^sub>1)) 
-      (com.Seq (Basic (\<lfloor>ncmp b\<rfloor>)) (lift\<^sub>c c\<^sub>2)))" |
-    "lift\<^sub>c (While b I c) = (com.Seq 
-      ((com.Seq (Basic (\<lfloor>cmp b\<rfloor>)) (lift\<^sub>c c))*) (Basic (\<lfloor>ncmp b\<rfloor>)))" |
-    "lift\<^sub>c (DoWhile I c b) = (com.Seq 
-      ((com.Seq (lift\<^sub>c c) (Basic (\<lfloor>cmp b\<rfloor>)))*) (com.Seq (lift\<^sub>c c) (Basic (\<lfloor>ncmp b\<rfloor>))))" |
-    "lift\<^sub>c (Test p) = Basic ((nop,tstate_rec.more), UNIV, {(m,m'). m = m' \<and> p m})" |
-    "lift\<^sub>c (Assert p) = Basic ((nop,tstate_rec.more), Collect p, Id)"
+      (com.Seq (Basic (\<lfloor>ncmp b\<rfloor>)) (lift\<^sub>c c\<^sub>2)))" 
 
-interpretation rules fwd\<^sub>s re\<^sub>a
-  by (unfold_locales) (auto simp: pred_defs)
+interpretation rules fwd\<^sub>s re\<^sub>a by (unfold_locales) (auto)
 
 abbreviation rules_abv ("_,_ \<turnstile> _ {_} _" [20,0,0,0,20] 20)
   where "rules_abv \<equiv> rules"
 
 abbreviation lifted_abv ("_,_,_ \<turnstile>\<^sub>s _ {_} _" [20,0,0,0,0,20] 20)
-  where "lifted_abv R G I P c Q \<equiv> \<langle>step\<^sub>t (inv I \<and>\<^sub>p R)\<rangle>,\<langle>step (inv I \<and>\<^sub>p G)\<rangle> \<turnstile> \<langle>all\<^sub>t I \<and>\<^sub>p P\<rangle> {lift\<^sub>c c} \<langle>all\<^sub>t I \<and>\<^sub>p Q\<rangle>"
+  where "lifted_abv R G I P c Q \<equiv> step\<^sub>t (inv I \<inter> R),step (inv I \<inter> G) \<turnstile> all\<^sub>t I \<inter> P {lift\<^sub>c c} all\<^sub>t I \<inter> Q"
 
 abbreviation validity_abv  ("\<Turnstile> _ SAT [_, _, _, _, _]" [60,0,0,0,0] 45) 
-  where "validity_abv c P R G Q I \<equiv> validity (lift\<^sub>c c) \<langle>all\<^sub>t I \<and>\<^sub>p P\<rangle> \<langle>step\<^sub>t (inv I \<and>\<^sub>p R)\<rangle> \<langle>step (inv I \<and>\<^sub>p G)\<rangle> \<langle>all\<^sub>t I \<and>\<^sub>p Q\<rangle>"
+  where "validity_abv c P R G Q I \<equiv> validity (lift\<^sub>c c) (all\<^sub>t I \<inter> P) (step\<^sub>t (inv I \<inter> R)) (step (inv I \<inter> G)) (all\<^sub>t I \<inter> Q)"
 
 text \<open>The language is always thread-local\<close>
 lemma local_lift [intro]:
@@ -225,105 +205,101 @@ lemma local_lift [intro]:
 
 text \<open>Correctness of the guarantee check\<close>
 lemma com_guar:
-  "wellformed R G \<Longrightarrow> guar\<^sub>c c G \<Longrightarrow> \<forall>\<beta>\<in>basics (lift\<^sub>c c). guar\<^sub>\<alpha> \<beta> \<langle>step G\<rangle>"
-  by (induct c) (auto simp: guar_def step_def reflexive_def wp_defs pred_defs liftl_def liftg_def)
-
+  "wellformed R G \<Longrightarrow> guar\<^sub>c c G \<Longrightarrow> \<forall>\<beta>\<in>basics (lift\<^sub>c c). guar\<^sub>\<alpha> \<beta> (step G)"
+  by (induct c) (auto simp: guar_def step_def reflexive_def wp\<^sub>r_def wp_CAS\<^sub>T_def wp_CAS_def wp_CAS\<^sub>F_def liftl_def liftg_def)
+ 
 text \<open>An ordering property on contexts\<close>
 definition context_order 
   ("_,_ \<turnstile>\<^sub>w _ \<ge> _" [100,0,0,100] 60)
   where "context_order R G P Q \<equiv> 
-    (stable\<^sub>t R Q \<and> wellformed R G) \<longrightarrow> ((P \<turnstile>\<^sub>p Q) \<and> stable\<^sub>t R P)"
+    (stable\<^sub>t R Q \<and> wellformed R G) \<longrightarrow> ((P \<subseteq> Q) \<and> stable\<^sub>t R P)"
 
 text \<open>The validity property we intend to show, abstracts over the preservation of wellformedness\<close>
 definition valid :: "('v,'a) grel \<Rightarrow> ('v,'a) grel \<Rightarrow> ('v,'a) gpred \<Rightarrow> ('v,'r,'a) pred \<Rightarrow> ('v,'r,'a) com_armv8 \<Rightarrow> ('v,'r,'a) pred \<Rightarrow> bool"
   ("_,_,_ \<turnstile>\<^sub>w _ {_} _" [100,0,0,0,0,100] 60)
   where "valid R G I P c Q \<equiv>  
-    (wellformed R G \<and> stable\<^sub>t R Q \<and> guar\<^sub>c c (inv I \<and>\<^sub>p G)) \<longrightarrow> (stable\<^sub>t R P \<and> (R,G,I \<turnstile>\<^sub>s P {c} Q))"
+    (wellformed R G \<and> stable\<^sub>t R Q \<and> guar\<^sub>c c (inv I \<inter> G)) \<longrightarrow> (stable\<^sub>t R P \<and> (R,G,I \<turnstile>\<^sub>s P {c} Q))"
 
 section \<open>Soundness\<close>
 
 subsection \<open>Sub-operations\<close>
 
 lemma stable\<^sub>t_local_op [intro!]:
-  "stable\<^sub>t R Q \<Longrightarrow> stable\<^sub>t R (\<lambda>m. Q (m\<lparr>rg := f (rg m)\<rparr>))"
-  by (auto simp add: stable_def step\<^sub>t_def)
+  assumes "stable\<^sub>t R Q" 
+  shows "stable\<^sub>t R {m. (m(Reg r :=\<^sub>s f (rg m))) \<in> Q}"
+  using assms by (auto simp: stable_def step\<^sub>t_def)
 
 lemma stable\<^sub>t_local_cmp [intro!]:
-  "stable\<^sub>t R Q \<Longrightarrow> stable\<^sub>t R (\<lambda>m. f (rg m) \<longrightarrow> Q m)"
+  "stable\<^sub>t R Q \<Longrightarrow> stable\<^sub>t R {m. f (rg m) \<longrightarrow> m \<in> Q}"
   by (auto simp add: stable_def step\<^sub>t_def)
-
-lemma stable\<^sub>t_local_assign [intro!]:
-  "stable\<^sub>t R Q \<Longrightarrow> stable\<^sub>t R (\<lambda>m. Q (m(r :=\<^sub>r f (rg m))))"
-  unfolding rg_upd_def by auto
 
 fun local_op
   where
     "local_op (load _ _) = False" |
-    "local_op (store _ _) = False" |
+    "local_op (cstore _ _ _) = False" |
     "local_op (cas\<^sub>T _ _ _) = False" |
-    "local_op (cas\<^sub>F _ _ _) = False" |
+    "local_op (cas\<^sub>F _ _) = False" |
     "local_op _ = True"
 
 lemma [intro]:
-  "(inv I) (m,m)"
+  "(m,m) \<in> inv I"
   by (auto simp: inv_def)
 
 lemma [intro!]:
-  "stable\<^sub>t R Q \<Longrightarrow> stable\<^sub>t ((\<lambda>(m, m'). I m \<longrightarrow> I m') \<and>\<^sub>p R) (\<lambda>m. I (glb m) \<and> Q m)"
+  "stable\<^sub>t R Q \<Longrightarrow> stable\<^sub>t ({(m, m'). m \<in> I \<longrightarrow> m' \<in> I} \<inter> R) ({m. glb m \<in> I} \<inter> Q)"
   by (auto simp: stable_def step\<^sub>t_def inv_def)
 
 lemma [intro!]:
-  "stable\<^sub>t R Q \<Longrightarrow> stable\<^sub>t (inv I \<and>\<^sub>p R) (all\<^sub>t I \<and>\<^sub>p Q)"
+  "stable\<^sub>t R Q \<Longrightarrow> stable\<^sub>t (inv I \<inter> R) (all\<^sub>t I \<inter> Q)"
   by (auto simp: stable_def step\<^sub>t_def inv_def all\<^sub>t_def)
 
 lemma [intro!]:
-  "reflexive G \<Longrightarrow> reflexive (inv I \<and>\<^sub>p G)"
+  "reflexive G \<Longrightarrow> reflexive (inv I \<inter> G)"
   by (auto simp: reflexive_def inv_def)
 
 text \<open>Basic Rule for global operations\<close>
 lemma basic_wp\<^sub>i_global:
-  assumes "P \<turnstile>\<^sub>p stabilize R (c \<and>\<^sub>p wp\<^sub>i \<alpha> (wp\<^sub>a a Q))" "wellformed R G" "stable\<^sub>t R Q" 
-  assumes "c \<turnstile>\<^sub>p guar (wp\<^sub>i \<alpha> o wp\<^sub>a a) (step (inv I \<and>\<^sub>p G))"
-  shows "\<langle>step\<^sub>t (inv I \<and>\<^sub>p R)\<rangle>,\<langle>step (inv I \<and>\<^sub>p G)\<rangle> \<turnstile> \<langle>all\<^sub>t I \<and>\<^sub>p P\<rangle> {Basic (\<lfloor>c, \<alpha>, a\<rfloor>)} \<langle>all\<^sub>t I \<and>\<^sub>p Q\<rangle>"
+  assumes "P \<subseteq> stabilize R (c \<inter> wp\<^sub>i \<alpha> (wp\<^sub>a a Q))" "wellformed R G" "stable\<^sub>t R Q" 
+  assumes "c \<subseteq> guar (wp\<^sub>i \<alpha> o wp\<^sub>a a) (step (inv I \<inter> G))"
+  shows "step\<^sub>t (inv I \<inter> R),step (inv I \<inter> G) \<turnstile> all\<^sub>t I \<inter> P {Basic (\<lfloor>c, \<alpha>, a\<rfloor>)} all\<^sub>t I \<inter> Q"
 proof -
-  have "\<langle>step\<^sub>t (inv I \<and>\<^sub>p R)\<rangle>,\<langle>step (inv I \<and>\<^sub>p G)\<rangle> \<turnstile>\<^sub>A \<langle>all\<^sub>t I \<and>\<^sub>p stabilize R (c \<and>\<^sub>p wp\<^sub>i \<alpha> (wp\<^sub>a a Q))\<rangle> {\<lfloor>c, \<alpha>, a\<rfloor>} \<langle>all\<^sub>t I \<and>\<^sub>p Q\<rangle>"
-    using assms by (cases \<alpha>) (auto simp: atomic_rule_def guar_def wp_def rg_upd_def 
-                                         step_def aux_upd_def pred_defs 
-                                         refl_def wp\<^sub>r_def o_def liftg_def all\<^sub>t_def inv_def
+  have "step\<^sub>t (inv I \<inter> R),step (inv I \<inter> G) \<turnstile>\<^sub>A all\<^sub>t I \<inter> stabilize R (c \<inter> wp\<^sub>i \<alpha> (wp\<^sub>a a Q)) {\<lfloor>c, \<alpha>, a\<rfloor>} all\<^sub>t I \<inter> Q"
+    using assms by (cases \<alpha>) (auto simp: atomic_rule_def guar_def wp_def 
+                                         step_def wp\<^sub>r_def o_def liftg_def all\<^sub>t_def inv_def
                                    elim!: stabilizeE)
-  thus ?thesis using assms by (intro conseq[OF basic]) (auto simp: pred_defs)
+  thus ?thesis using assms by (intro conseq[OF basic]) (auto)
 qed
 
 text \<open>Basic Rule for local operations\<close>
 lemma basic_wp\<^sub>i_local:
-  assumes "P \<turnstile>\<^sub>p wp\<^sub>i \<alpha> Q" "wellformed R G" "stable\<^sub>t R Q" "local_op \<alpha>" 
-  shows "\<langle>step\<^sub>t (inv I \<and>\<^sub>p R)\<rangle>,\<langle>step (inv I \<and>\<^sub>p G)\<rangle> \<turnstile> \<langle>all\<^sub>t I \<and>\<^sub>p P\<rangle> {Basic (\<lfloor>\<alpha>\<rfloor>)} \<langle>all\<^sub>t I \<and>\<^sub>p Q\<rangle>"
+  assumes "P \<subseteq> wp\<^sub>i \<alpha> Q" "wellformed R G" "stable\<^sub>t R Q" "local_op \<alpha>" 
+  shows "step\<^sub>t (inv I \<inter> R),step (inv I \<inter> G) \<turnstile> all\<^sub>t I \<inter> P {Basic (\<lfloor>\<alpha>\<rfloor>)} all\<^sub>t I \<inter> Q"
 proof -
-  have "\<langle>step\<^sub>t (inv I \<and>\<^sub>p R)\<rangle>,\<langle>step (inv I \<and>\<^sub>p G)\<rangle> \<turnstile>\<^sub>A  \<langle>all\<^sub>t I \<and>\<^sub>p wp\<^sub>i \<alpha> Q\<rangle> {\<lfloor>\<alpha>\<rfloor>} \<langle>all\<^sub>t I \<and>\<^sub>p Q\<rangle>"
-    using assms by (cases \<alpha>) (auto simp: atomic_rule_def guar_def wp_def rg_upd_def 
-                                         step_def aux_upd_def pred_defs liftl_def all\<^sub>t_def inv_def
+  have "step\<^sub>t (inv I \<inter> R),step (inv I \<inter> G) \<turnstile>\<^sub>A  all\<^sub>t I \<inter> wp\<^sub>i \<alpha> Q {\<lfloor>\<alpha>\<rfloor>} all\<^sub>t I \<inter> Q"
+    using assms by (cases \<alpha>) (auto simp: atomic_rule_def guar_def wp_def reflexive_def
+                                         step_def liftl_def all\<^sub>t_def inv_def
                                          elim!: stabilizeE)
-  thus ?thesis using assms by (intro conseq[OF basic]) (auto simp: pred_defs)
+  thus ?thesis using assms by (intro conseq[OF basic]) (auto)
 qed
 
 text \<open>Automation to assist with Load/Store/CAS\<close>
 lemma stabilize_cmp:
-  "P \<turnstile>\<^sub>p wp\<^sub>i (cmp b) Q \<Longrightarrow> stabilize R P \<turnstile>\<^sub>p wp\<^sub>i (cmp b) (stabilize R Q)"
-  by (auto simp: pred_defs stabilize_def set_glb_def)
+  "P \<subseteq> wp\<^sub>i (cmp b) Q \<Longrightarrow> stabilize R P \<subseteq> wp\<^sub>i (cmp b) (stabilize R Q)"
+  by (auto simp: stabilize_def)
 
 method expand_seq =
   (clarsimp, intro rules.choice rules.seqset; (clarsimp, intro rules.ord, (auto)[1]))
 
 method basic_wp\<^sub>i = 
   ((rule basic_wp\<^sub>i_local | rule basic_wp\<^sub>i_global), 
-   (rule stabilize_cmp | blast); 
-   auto simp: wp_defs pred_defs step_def aux_upd_def)
+   (rule stabilize_cmp | rule subset_refl); 
+   auto simp: wp\<^sub>r_def step_def wp_CAS_def wp_CAS\<^sub>T_def wp_CAS\<^sub>F_def)
 
 text \<open>A rule for cmp operations, used for If/While/DoWhile\<close>
 lemma cmp_sound [intro!]:
   assumes "wellformed R G" "stable\<^sub>t R Q"
-  assumes "P \<turnstile>\<^sub>p wp\<^sub>i (cmp b) Q"
-  shows "\<langle>step\<^sub>t (inv I \<and>\<^sub>p R)\<rangle>,\<langle>step (inv I \<and>\<^sub>p G)\<rangle> \<turnstile> \<langle>all\<^sub>t I \<and>\<^sub>p P\<rangle> {Basic (\<lfloor>cmp b\<rfloor>)} \<langle>all\<^sub>t I \<and>\<^sub>p Q\<rangle>"
+  assumes "P \<subseteq> wp\<^sub>i (cmp b) Q"
+  shows "step\<^sub>t (inv I \<inter> R),step (inv I \<inter> G) \<turnstile> all\<^sub>t I \<inter> P {Basic (\<lfloor>cmp b\<rfloor>)} all\<^sub>t I \<inter> Q"
   using assms by (intro basic_wp\<^sub>i_local) auto
 
 subsection \<open>State Ordering\<close>
@@ -333,16 +309,16 @@ text \<open>Properties of the state ordering. Essentially entailment with preser
 text \<open>The ordering is reflexive\<close>
 lemma refl_ord:
   "R,G \<turnstile>\<^sub>w P \<ge> P"
-  unfolding context_order_def by (auto simp: pred_defs)
+  unfolding context_order_def by auto
 
 text \<open>It is possible to strengthen the RHS\<close>
 lemma assert_ord:
-  "R,G \<turnstile>\<^sub>w P \<and>\<^sub>p assert A \<ge> P"
-  by (cases A) (auto simp: pred_defs context_order_def assert_def) 
+  "R,G \<turnstile>\<^sub>w P \<inter> assert A \<ge> P"
+  by (cases A) (auto simp: context_order_def assert_def) 
 
 text \<open>Stabilize Ordering\<close>
 lemma stabilize_ord [intro]:
-  assumes "P \<turnstile>\<^sub>p Q" 
+  assumes "P \<subseteq> Q" 
   shows "R,G \<turnstile>\<^sub>w stabilize R P \<ge> Q"
   using assms stabilizeE unfolding context_order_def 
   by blast
@@ -351,59 +327,25 @@ subsection \<open>Rules\<close>
 
 text \<open>If Rule\<close>
 lemma if_wp:
-  "R,G,I \<turnstile>\<^sub>w P\<^sub>1 {c\<^sub>1} Q \<Longrightarrow> R,G,I \<turnstile>\<^sub>w P\<^sub>2 {c\<^sub>2} Q \<Longrightarrow> R,G,I \<turnstile>\<^sub>w wp\<^sub>i (cmp b) P\<^sub>1 \<and>\<^sub>p wp\<^sub>i (ncmp b) P\<^sub>2 {If b c\<^sub>1 c\<^sub>2} Q"
-  unfolding valid_def by clarsimp (intro conjI rules.choice rules.seq, auto simp add: pred_defs)
-
-text \<open>While Rule\<close>
-lemma while_wp:
-  assumes "R,G,I \<turnstile>\<^sub>w P {c} stabilize R J" (is "R,G,I \<turnstile>\<^sub>w P {c} ?I")
-  assumes "J \<turnstile>\<^sub>p wp\<^sub>i (cmp b) P \<and>\<^sub>p wp\<^sub>i (ncmp b) Q"
-  shows "R,G,I \<turnstile>\<^sub>w ?I {While b J c} Q"
-  unfolding valid_def lift\<^sub>c.simps
-proof (intro impI conjI rules.choice rules.seq)
-  assume "wellformed R G \<and> stable\<^sub>t R Q \<and> guar\<^sub>c (While b J c) (inv I \<and>\<^sub>p G)"
-  thus "\<langle>step\<^sub>t (inv I \<and>\<^sub>p R)\<rangle>,\<langle>step (inv I \<and>\<^sub>p G)\<rangle> \<turnstile> \<langle>all\<^sub>t I \<and>\<^sub>p ?I\<rangle> {(Basic (\<lfloor>cmp b\<rfloor>) ;; lift\<^sub>c c)*} \<langle>all\<^sub>t I \<and>\<^sub>p ?I\<rangle>"
-    using assms 
-    apply (intro rules.loop rules.seq, unfold valid_def)
-    apply force
-    apply force
-    by (auto simp: pred_defs elim!: stabilizeE)
-qed (insert assms, auto simp add: pred_defs elim!: stabilizeE)
-
-text \<open>Do While Rule\<close>
-lemma do_wp:
-  assumes "R,G,I \<turnstile>\<^sub>w stabilize R J {c} (wp\<^sub>i (cmp b) (stabilize R J) \<and>\<^sub>p wp\<^sub>i (ncmp b) Q)" (is "R,G,I \<turnstile>\<^sub>w ?I {c} ?Q")
-  shows "R,G,I \<turnstile>\<^sub>w stabilize R J {DoWhile J c b} Q"
-  unfolding valid_def lift\<^sub>c.simps
-proof (intro impI conjI rules.choice rules.seq)
-  assume "wellformed R G \<and> stable\<^sub>t R Q \<and> guar\<^sub>c (DoWhile J c b) (inv I \<and>\<^sub>p G)"
-  thus "\<langle>step\<^sub>t (inv I \<and>\<^sub>p R)\<rangle>,\<langle>step (inv I \<and>\<^sub>p G)\<rangle> \<turnstile> \<langle>all\<^sub>t I \<and>\<^sub>p ?I\<rangle> {lift\<^sub>c c} \<langle>all\<^sub>t I \<and>\<^sub>p ?Q\<rangle>" 
-    using assms by (auto simp: valid_def) 
-next
-  assume "wellformed R G \<and> stable\<^sub>t R Q \<and> guar\<^sub>c (DoWhile J c b) (inv I \<and>\<^sub>p G)"
-  thus "\<langle>step\<^sub>t (inv I \<and>\<^sub>p R)\<rangle>,\<langle>step (inv I \<and>\<^sub>p G)\<rangle> \<turnstile> \<langle>all\<^sub>t I \<and>\<^sub>p ?I\<rangle> {(lift\<^sub>c c ;; Basic (\<lfloor>cmp b\<rfloor>))*} \<langle>all\<^sub>t I \<and>\<^sub>p ?I\<rangle>"
-    using assms 
-    apply (intro rules.loop seq_rot)
-    apply (auto simp: valid_def)[2]
-    by (auto simp: pred_defs)
-qed (insert assms, auto simp add: pred_defs)
+  "R,G,I \<turnstile>\<^sub>w P\<^sub>1 {c\<^sub>1} Q \<Longrightarrow> R,G,I \<turnstile>\<^sub>w P\<^sub>2 {c\<^sub>2} Q \<Longrightarrow> R,G,I \<turnstile>\<^sub>w wp\<^sub>i (cmp b) P\<^sub>1 \<inter> wp\<^sub>i (ncmp b) P\<^sub>2 {If b c\<^sub>1 c\<^sub>2} Q"
+  unfolding valid_def by clarsimp (intro conjI rules.choice rules.seq, auto)
 
 text \<open>False Rule\<close>
 lemma false_wp:
-  assumes "P \<turnstile>\<^sub>p (\<lambda>m. False)"
+  assumes "P \<subseteq> {}"
   shows "R,G,I \<turnstile>\<^sub>w P {c} Q"
   using assms unfolding valid_def
-  by (intro conjI impI com_guar rules.conseq[OF falseI, where ?G="\<langle>step (inv I \<and>\<^sub>p G)\<rangle>"]) (auto simp: pred_defs)
+  by (intro conjI impI com_guar rules.conseq[OF falseI, where ?G="step (inv I \<inter> G)"]) (auto)
 
 text \<open>Rewrite Rule\<close>
 lemma rewrite_wp:
   "R,G,I \<turnstile>\<^sub>w P {c} Q \<Longrightarrow> R,G \<turnstile>\<^sub>w M \<ge> P \<Longrightarrow> R,G,I \<turnstile>\<^sub>w M {c} Q"
-  by (auto simp: pred_defs valid_def context_order_def)
+  by (auto simp: valid_def context_order_def)
 
 text \<open>Assert Rule\<close>
 lemma assert_wp:
   assumes "A \<Longrightarrow> R,G,I \<turnstile>\<^sub>w P {c} Q"
-  shows "R,G,I \<turnstile>\<^sub>w (P \<and>\<^sub>p assert A) {c} Q"
+  shows "R,G,I \<turnstile>\<^sub>w (P \<inter> assert A) {c} Q"
 proof (cases A)
   case True
   then show ?thesis using assms by (intro rewrite_wp[OF _ assert_ord], simp)
@@ -411,6 +353,10 @@ next
   case False
   then show ?thesis by (intro false_wp, auto simp: assert_def)
 qed 
+
+lemma [simp]:
+  "m(aux: \<lambda>m. f (m(x :=\<^sub>s e)), x :=\<^sub>s e) = m(x :=\<^sub>s e, aux: f)"
+  by (auto simp: aux_upd_def st_upd_def)
 
 text \<open>Com Rule\<close>
 theorem com_wp:
@@ -421,17 +367,7 @@ proof (induct c arbitrary: Q)
 next
   case (Op r e)
   thus ?case unfolding valid_def lift\<^sub>c.simps 
-    by (intro conjI impI basic_wp\<^sub>i_local) (auto simp: rg_upd_def)
-next
-  case (Test p)
-  thus ?case unfolding valid_def lift\<^sub>c.simps
-    by (intro conjI impI rules.basic)
-       (auto simp: atomic_rule_def wp_def pred_defs guar_def step_def elim!: stabilizeE)
-next
-  case (Assert p)
-  thus ?case unfolding valid_def lift\<^sub>c.simps
-    by (intro conjI impI rules.basic)
-       (auto simp: atomic_rule_def wp_def pred_defs guar_def step_def elim!: stabilizeE)
+    by (intro conjI impI basic_wp\<^sub>i_local) (auto)
 next
   case (Load c r\<^sub>a r a)
   thus ?case unfolding valid_def by (intro conjI impI, force) (expand_seq, basic_wp\<^sub>i+)
@@ -444,12 +380,6 @@ next
 next
   case (If b c\<^sub>1 c\<^sub>2)
   thus ?case unfolding wp.simps wpre.simps by (blast intro: if_wp)
-next
-  case (While b I c)
-  thus ?case unfolding wp.simps by (intro assert_wp impI while_wp) (auto simp: pred_defs)
-next
-  case (DoWhile I c b)
-  thus ?case unfolding wp.simps by (intro assert_wp do_wp; rule rewrite_wp) auto
 qed (auto simp: valid_def)
 
 subsection \<open>High-Level Theorem\<close>
@@ -458,12 +388,12 @@ text \<open>Soundness lemma for WP reasoning over ARMv8\<close>
 theorem armv8_wp_sound:
   assumes wf: "transitive R" "reflexive R" "reflexive G" 
   assumes st: "stable\<^sub>t R Q" 
-  assumes g: "guar\<^sub>c c (inv I \<and>\<^sub>p G)"
-  assumes P: "P \<turnstile>\<^sub>p wp R c Q"
+  assumes g: "guar\<^sub>c c (inv I \<inter> G)"
+  assumes P: "P \<subseteq> wp R c Q"
   shows "\<Turnstile> c SAT [P, R, G, Q, I]"
 proof -
   have "R,G,I \<turnstile>\<^sub>s wp R c Q {c} Q" using wf st g com_wp unfolding valid_def by blast
-  hence "R,G,I \<turnstile>\<^sub>s P {c} Q" by (rule rules.conseq) (insert P, auto simp: pred_defs)
+  hence "R,G,I \<turnstile>\<^sub>s P {c} Q" by (rule rules.conseq) (insert P, auto)
   thus ?thesis by (intro sound thread) auto
 qed
 
