ARMv8/ARMv8_State.thy
@@ -4,38 +4,52 @@ begin
 
 section \<open>State Encoding\<close>
 
-record 'v gstate_rec = st :: "'v \<Rightarrow> 'v"
-record ('v,'r) tstate_rec = "'v gstate_rec" + rg :: "'r \<Rightarrow> 'v"
+datatype ('v,'r) var = Reg 'r | Glb 'v
+record ('v,'a) state_rec = st :: "'a \<Rightarrow> 'v"
 
-type_synonym ('v,'r,'a) tstate = "('v,'r,'a) tstate_rec_scheme"
-type_synonym ('v,'a) gstate = "('v,'a) gstate_rec_scheme"
+type_synonym ('v,'r,'a) state = "('v,('v,'r) var,'a) state_rec_scheme"
+type_synonym ('v,'a) gstate = "('v,'v,'a) state_rec_scheme"
 
-type_synonym ('v,'r,'a) pred = "('v,'r,'a) tstate \<Rightarrow> bool"
-type_synonym ('v,'a) gpred = "('v,'a) gstate \<Rightarrow> bool"
+type_synonym ('v,'r,'a) pred = "('v,'r,'a) state set"
+type_synonym ('v,'a) gpred = "('v,'a) gstate set"
 
-type_synonym ('v,'r,'a) trel = "(('v,'r,'a) tstate \<times> ('v,'r,'a) tstate) \<Rightarrow> bool"
-type_synonym ('v,'a) grel = "(('v,'a) gstate \<times> ('v,'a) gstate) \<Rightarrow> bool"
+type_synonym ('v,'r,'a) trel = "('v,'r,'a) state rel"
+type_synonym ('v,'a) grel = "('v,'a) gstate rel"
+
 type_synonym ('v,'r,'a) trans = "('v,'r,'a) pred \<Rightarrow> ('v,'r,'a) pred"
 type_synonym ('v,'r,'a) rtrans = "('v,'r,'a) trel \<Rightarrow> ('v,'r,'a) trel"
 
-type_synonym ('v,'r,'a) auxfn = "('v,'r,'a) tstate \<Rightarrow> 'a"
+type_synonym ('v,'r,'a) auxfn = "('v,('v,'r) var,'a) state_rec_scheme \<Rightarrow> 'a"
+
+definition glb
+  where "glb m \<equiv> \<lparr> st = (\<lambda>v. st m (Glb v)), \<dots> = more m \<rparr>"
+
+definition rg :: "('v,'r,'a) state \<Rightarrow> ('r \<Rightarrow> 'v)"
+  where "rg m \<equiv> \<lambda>v. st m (Reg v)"
+
+definition aux
+  where "aux m \<equiv> more m"
+
+text \<open>Domain of register variables\<close>
+abbreviation locals
+  where "locals \<equiv> Reg ` UNIV"
+
+text \<open>Domain of register variables\<close>
+abbreviation globals
+  where "globals \<equiv> Glb ` UNIV"
 
 section \<open>Write Operations\<close>
 
-definition st_upd :: "('v,'a) gstate \<Rightarrow> 'v \<Rightarrow> 'v \<Rightarrow> ('v,'a) gstate"
+definition st_upd :: "('v,'a,'b) state_rec_scheme \<Rightarrow> 'a \<Rightarrow> 'v \<Rightarrow> ('v,'a,'b) state_rec_scheme"
   where "st_upd m a b = m \<lparr> st := ((st m) (a := b)) \<rparr>"
 
-definition rg_upd :: "('v,'r,'a) tstate \<Rightarrow> 'r \<Rightarrow> 'v \<Rightarrow> ('v,'r,'a) tstate"
-  where "rg_upd m a b = m \<lparr> rg := ((rg m) (a := b)) \<rparr>"
-
-definition aux_upd :: "('v,'r,'a) tstate \<Rightarrow> ('v,'r,'a) auxfn \<Rightarrow> ('v,'r,'a) tstate"
-  where "aux_upd m f \<equiv> m\<lparr>tstate_rec.more := f m\<rparr>"
+definition aux_upd :: "('v,'r,'a) state_rec_scheme \<Rightarrow> (('v,'r,'a) state_rec_scheme \<Rightarrow> 'a) \<Rightarrow> ('v,'r,'a) state_rec_scheme"
+  where "aux_upd m f \<equiv> m\<lparr>state_rec.more := f m\<rparr>"
 
 nonterminal updbinds and updbind
 
 syntax
   "_updbindm" :: "'a \<Rightarrow> 'a \<Rightarrow> updbind"            ("(2_ :=\<^sub>s/ _)")
-  "_updbindr" :: "'a \<Rightarrow> 'a \<Rightarrow> updbind"            ("(2_ :=\<^sub>r/ _)")
   "_updbinda" :: "'a \<Rightarrow> updbind"                  ("(2aux:/ _)")
   ""         :: "updbind \<Rightarrow> updbinds"             ("_")
   "_updbinds":: "updbind \<Rightarrow> updbinds \<Rightarrow> updbinds" ("_,/ _")
@@ -43,115 +57,61 @@ syntax
 
 translations
   "_Update f (_updbinds b bs)" \<rightleftharpoons> "_Update (_Update f b) bs"
-  "f(x:=\<^sub>ry)" \<rightleftharpoons> "CONST rg_upd f x y"
   "f(x:=\<^sub>sy)" \<rightleftharpoons> "CONST st_upd f x y"
   "f(aux: y)" \<rightleftharpoons> "CONST aux_upd f y"
 
-definition glb :: "('v,'r,'a) tstate \<Rightarrow> ('v,'a) gstate"
-  where "glb m \<equiv> \<lparr> st = st m, \<dots> = more m \<rparr>"
+section \<open>Simp Lemmas\<close>
 
-definition set_glb :: "('v,'r,'a) tstate \<Rightarrow> ('v,'a) gstate \<Rightarrow> ('v,'r,'a) tstate"
-  where "set_glb m g \<equiv> \<lparr> st = st g, rg = rg m, \<dots> = gstate_rec.more g \<rparr>"
+lemma aux_nop [simp]:
+  "m(aux:aux) = m"
+  by (auto simp: aux_def aux_upd_def)
 
-lemma [simp]:
-  "set_glb m (glb m) = m"
-  by (auto simp: set_glb_def glb_def)
-
-section \<open>Simple Predicate Encoding\<close>
-
-named_theorems pred_defs
-
-abbreviation conj  (infixr "\<and>\<^sub>p" 35)
-  where "conj l r \<equiv> \<lambda>m. (l m) \<and> (r m)"
-
-abbreviation disj  (infixr "\<or>\<^sub>p" 35)
-  where "disj l r \<equiv> \<lambda>m. (l m) \<or> (r m)"
-
-abbreviation imp  (infixr "\<longrightarrow>\<^sub>p" 35)
-  where "imp l r \<equiv> \<lambda>m. (l m) \<longrightarrow> (r m)"
-
-definition entail (infix "\<turnstile>\<^sub>p" 25)
-  where "entail P Q \<equiv> \<forall>m. P m \<longrightarrow> Q m"
-
-declare entail_def [pred_defs]
-
-definition assert
-  where "assert b \<equiv> \<lambda>m. b"
-
-abbreviation True\<^sub>p
-  where "True\<^sub>p \<equiv> \<lambda>m. True"
-
-lemma [simp]:
-  "(P \<turnstile>\<^sub>p P) = True"
-  by (auto simp add: pred_defs)
-
-lemma [simp]:
-  "(P \<and>\<^sub>p P) = P"
-  by (auto simp: pred_defs)
-
-section \<open>Base Definitions for Relations\<close>
-
-definition reflexive 
-  where "reflexive R \<equiv> \<forall>m . R (m,m)"
-
-definition transitive 
-  where "transitive R \<equiv> \<forall>m m' m''. R (m,m') \<longrightarrow> R (m',m'') \<longrightarrow> R (m,m'')"
-
-definition stabilize :: "('v,'a) grel \<Rightarrow> ('v,'r,'a) pred \<Rightarrow> ('v,'r,'a) pred"
-  where "stabilize R P \<equiv> \<lambda>m. \<forall>g. R (glb m,g) \<longrightarrow> P (set_glb m g)"
-
-section \<open>Simp\<close>
-
-lemma [simp]:
-  "rg (set_glb m g) r\<^sub>a = rg m r\<^sub>a"
-  by (auto simp: set_glb_def)
-
-lemma [simp]:
-  "set_glb (set_glb m g) g' = set_glb m g'"
-  by (auto simp: set_glb_def)
-
-lemma [simp]:
-  "set_glb (m\<lparr>tstate_rec.more := a\<rparr>) g = set_glb m g"
-  by (auto simp: set_glb_def)
-
-lemma [simp]:
-  "st (set_glb m g) = st g"
-  by (auto simp: set_glb_def)
-
-lemma [simp]:
-  "\<forall>m. \<not> P m \<Longrightarrow> Collect P = {}"
-  by (auto)
-
-lemma [simp]:
-  "glb (m\<lparr>rg := e\<rparr>) = glb m"
-  unfolding glb_def by auto
-
-lemma [simp]:
-  "m(r :=\<^sub>r e)\<lparr>tstate_rec.more := a\<rparr> = (m\<lparr>tstate_rec.more := a\<rparr>)(r :=\<^sub>r e)"
-  by (auto simp: rg_upd_def)
-
-lemma [simp]:
-  "glb (m(r :=\<^sub>r T)) = glb m"
-  by (auto simp: glb_def rg_upd_def)
-
-lemma [simp]:
-  "m(aux: tstate_rec.more) = m"
+lemma aux_st [simp]:
+  "st (m(aux: e)) = st m"
   by (auto simp: aux_upd_def)
 
 lemma [simp]:
-  "glb (set_glb m g) = g"
-  by (auto simp: glb_def set_glb_def)
+  "st (m(r :=\<^sub>s e)) q = (if r = q then e else st m q)"
+  by (auto simp: st_upd_def)
 
 lemma [simp]:
-  "glb (x(x3 :=\<^sub>r e, aux: x4)) = glb (x(aux: \<lambda>m. x4 (m(x3 :=\<^sub>r e))))"
-  by (auto simp: rg_upd_def aux_upd_def glb_def)
+  "st (m(v :=\<^sub>s e)) = (st m)(v := e)"
+  by (auto simp: st_upd_def)
 
-lemma [intro]:
-  "reflexive G \<Longrightarrow> G (m,m)"
-  by (auto simp: reflexive_def)
+lemma [simp]:
+  "more (m(r :=\<^sub>s e)) = more m"
+  by (auto simp: st_upd_def)
 
-lemma entail_refl [intro]:
-  "P \<turnstile>\<^sub>p P"
-  by (auto simp: pred_defs)
+lemma [simp]:
+  "more (m(aux: e)) = e m"
+  by (auto simp: aux_upd_def)
+
+lemma [simp]:
+  "rg (m(Glb x :=\<^sub>s e)) = rg m"
+  by (auto simp: rg_def st_upd_def)
+
+lemma [simp]:
+  "rg (m(Reg x :=\<^sub>s e)) = (rg m)(x := e)"
+  by (auto simp: st_upd_def rg_def)
+
+lemma [simp]:
+  "glb (m(Reg r :=\<^sub>s e)) = glb m"
+  by (auto simp: glb_def st_upd_def)
+
+lemma [simp]:
+  "glb (m(Reg r :=\<^sub>s e, aux: f)) = glb (m(aux: \<lambda>m. f(m(Reg r :=\<^sub>s e))))"
+  by (auto simp: aux_def glb_def)
+
+lemma [simp]:
+  "st m (Reg x) = rg m x"
+  by (auto simp: rg_def)
+
+lemma [simp]:
+  "glb (m(Reg x :=\<^sub>s e)) = glb m"
+  by (auto simp: glb_def st_upd_def)
+
+lemma [simp]:
+  "aux (m(Reg x :=\<^sub>s e)) = aux m"
+  by (auto simp: aux_def st_upd_def)
 
 end
