ARMv8/ARMv8_Inter.thy
@@ -1,0 +1,1208 @@
+theory ARMv8_Inter
+  imports ARMv8_Rules
+begin
+
+text \<open>
+This theory file describes the abstract interference pairs analysis
+and includes a soundness proof.
+\<close>
+
+abbreviation inst
+  where "inst a \<equiv> fst (fst a)"
+
+text \<open>The abstract language features used by liftc\<close>
+fun sim :: "('a,'b) com \<Rightarrow> bool"
+  where 
+    "sim (c\<^sub>1 || c\<^sub>2) = False" |
+    "sim (Thread _) = False" |
+    "sim (c*) = False" |   
+    "sim (c\<^sub>1 \<cdot> c\<^sub>2) = (sim c\<^sub>1 \<and> sim c\<^sub>2)" |
+    "sim (c\<^sub>1 ;; c\<^sub>2) = (sim c\<^sub>1 \<and> sim c\<^sub>2)" |
+    "sim (c\<^sub>1 \<sqinter> c\<^sub>2) = (sim c\<^sub>1 \<and> sim c\<^sub>2)" |  
+    "sim _ = True"
+
+definition wfbasic :: "('v,'r,'a) subbasic \<Rightarrow> bool"
+  where "wfbasic \<beta> \<equiv> beh \<beta> = beh\<^sub>a (tag \<beta>) \<and> (case inst \<beta> of cfence \<Rightarrow> vc \<beta> = UNIV \<and> beh \<beta> = beh\<^sub>i cfence | _ \<Rightarrow> True)"
+
+definition wfcom
+  where "wfcom c \<equiv> \<forall>\<beta> \<in> basics c. wfbasic \<beta>"
+
+text \<open>The language is always thread-local\<close>
+lemma sim_lift [intro]:
+  "sim (lift\<^sub>c c)"
+  by (induct c) auto
+
+lemma sim_seq2com [intro]:
+  "sim (seq2com s)"
+  by (induct s) auto
+
+lemma sim_silent:
+  "c \<leadsto> c' \<Longrightarrow> sim c \<Longrightarrow> sim c'"
+  by (induct rule: silent.induct) auto
+
+lemma sim_execute:
+  "lexecute c r \<alpha> c' \<Longrightarrow> sim c \<Longrightarrow> sim c'"
+  by (induct rule: lexecute.induct) auto
+
+lemma sim_prefix:
+  "lexecute c r \<alpha> c' \<Longrightarrow> sim c \<Longrightarrow> sim r"
+  by (induct rule: lexecute.induct, auto)
+
+lemma aux_exec [intro!]:
+  assumes "(m\<^sub>1,m\<^sub>2) \<in> P"
+  shows "(m\<^sub>1,m\<^sub>2(aux: f)) \<in> P O {(m, m'). m' = m(aux: f)}"
+  using assms by blast
+
+lemma [simp]:
+  "P O {(m, m'). m' = m} = P"
+  by auto
+
+lemma wfcomI [intro]:
+  "wfcom (lift\<^sub>c c)"
+  by (induct c) (auto simp: wfcom_def wfbasic_def liftg_def liftl_def)
+
+lemma [simp]:
+  "wfcom (c\<^sub>1 ;; c\<^sub>2) = (wfcom c\<^sub>1 \<and> wfcom c\<^sub>2)"
+  by (auto simp: wfcom_def)
+
+lemma [simp]:
+  "wfcom (Ord c\<^sub>1 c\<^sub>2) = (wfcom c\<^sub>1 \<and> wfcom c\<^sub>2)"
+  by (auto simp: wfcom_def)
+
+lemma wfcom_silent:
+  "c \<leadsto> c' \<Longrightarrow> wfcom c \<Longrightarrow> wfcom c'"
+  using basics_silent by (auto simp: wfcom_def)
+
+lemma wfcom_exec:
+  "lexecute c r \<alpha> c' \<Longrightarrow> wfcom c \<Longrightarrow> wfcom c'"
+  using basics_exec unfolding wfcom_def by blast
+
+lemma wfcom_exec_prefix:
+  "lexecute c r \<alpha> c' \<Longrightarrow> wfcom c \<Longrightarrow> wfcom r \<and> wfbasic \<alpha>"
+  using basics_exec_prefix unfolding wfcom_def by blast
+
+lemma opbasicE:
+  obtains (op) x e f v b where  "(basic ) = ((op x e,f), v, b)" |
+          (cmp) g f v b where "(basic ) = ((cmp g,f), v, b)" |
+          (fence) f v b where "(basic ) = ((fence,f), v, b)" |
+          (cfence) f v b where "(basic ) = ((cfence,f), v, b)" |
+          (stfence) f v b where "(basic ) = ((stfence,f), v, b)" |
+          (load) x e f v b where "(basic ) = ((load x e,f), v, b)" |
+          (store) b x e f v h where "(basic ) = ((cstore b x e,f), v, h)" |
+          (cas\<^sub>T) x e1 e2 f v b where "(basic ) = ((cas\<^sub>T x e1 e2,f), v, b)" |
+          (cas\<^sub>F) x e1 f v b where "(basic ) = ((cas\<^sub>F x e1,f), v, b)" |
+          (nop) f v b where "(basic ) = ((nop,f), v, b)" 
+  by (cases basic, case_tac a, case_tac aa; clarsimp)
+
+lemma fwd_wfbasic:
+  assumes "reorder_com \<alpha>' r \<alpha>" "wfbasic \<alpha>" 
+  shows "wfbasic \<alpha>'"
+  using assms
+proof (induct \<alpha>' r \<alpha> rule: reorder_com.induct)
+  case (2 \<alpha>' \<beta> \<alpha>)
+  then show ?case by (cases \<alpha> rule: opbasicE; cases \<beta> rule: opbasicE; auto simp: Let_def wfbasic_def)
+qed auto
+
+lemma fwdE:
+  assumes "reorder_inst \<alpha>' \<beta> \<alpha>"
+  obtains (no_fwd) "inst \<alpha>' = inst \<alpha>" "snd (tag \<alpha>') = snd (tag \<alpha>)" "vc \<alpha>' = vc \<alpha>" "wr (inst \<beta>) \<inter> rd (inst \<alpha>) = {}" |
+          (fwd) x where "wr (inst \<beta>) = {x}" "x \<in> rd (inst \<alpha>)" "rd (inst \<beta>) - {x} \<subseteq> locals"
+proof (cases "wr (inst \<beta>) \<inter> rd (inst \<alpha>) = {}")
+  case True
+  then show ?thesis using no_fwd assms    
+    by (cases \<alpha> rule: opbasicE; cases \<beta> rule: opbasicE; auto simp: Let_def split: if_splits)
+next
+  case False
+  then show ?thesis using fwd assms 
+    by (cases \<alpha> rule: opbasicE; cases \<beta> rule: opbasicE; auto simp: Let_def split: if_splits)
+qed
+
+fun exp
+  where 
+    "exp (subop.op x e) = e" | 
+    "exp (subop.cstore b x e) = e" | 
+    "exp (subop.cas\<^sub>T x e\<^sub>1 e\<^sub>2) = e\<^sub>2" | 
+    "exp _ = undefined"
+
+section \<open>Definitions\<close>
+
+text \<open>
+A data point, extends an instruction with reordering information.
+Forms the basis of the analysis, as each instruction generates a point that is maintained
+across all instructions earlier to it in program-order.
+Collects the transitive dependencies of said instruction along with all instructions
+it may reorder with.
+Moreover, it collects those variables that may be redefined between the two (esc) two
+handle forwarding manipulations.
+\<close>
+record ('v,'r,'a) point =
+  op :: "('v,'r,'a) subbasic"
+  wrs :: "('v,'r) var set"
+  rds :: "('v,'r) var set"
+  bar :: "('v,'r) subop set"
+  esc :: "('v,'r) var set"
+  pairs :: "(('v,'r,'a) subbasic \<times> ('v,'r) var set) set"
+
+type_synonym ('v,'r,'a) points = "('v,'r,'a) point set"
+
+subsection \<open>Tests\<close>
+
+text \<open>Test if a set contains a global variable\<close>
+definition hasGlobal :: "('g,'r) var set \<Rightarrow> bool"
+  where "hasGlobal S \<equiv> \<exists>e. Glb e \<in> S"
+
+
+text \<open>Test if a point is dependent on an operation, implying ordering of their execution\<close>
+fun ord :: "('v,'r) subop \<Rightarrow> ('v,'r,'a) point \<Rightarrow> bool"
+  where
+    "ord fence _ = True" |
+    "ord nop p = (fence \<in> bar p)" |
+    "ord stfence p = (fence \<in> bar p \<or> hasGlobal (wrs p))" |
+    "ord cfence p = (fence \<in> bar p \<or> hasGlobal (rds p))" |
+    "ord (cmp b) p = (fence \<in> bar p \<or> cfence \<in> bar p \<or> hasGlobal (wrs p) \<or> wrs p \<inter> rd (cmp b) \<noteq> {})" |
+    "ord (cstore b a e) p = (fence \<in> bar p \<or> stfence \<in> bar p \<or> Glb a \<in> wrs p)" |
+    "ord (subop.op r e) p = (fence \<in> bar p \<or> Reg r \<in> wrs p)" |
+    "ord (load a e) p = (fence \<in> bar p \<or> Glb a \<in> wrs p \<or> Glb a \<in> rds p)" |
+    "ord (cas\<^sub>T a e\<^sub>1 e\<^sub>2) p = (fence \<in> bar p \<or> stfence \<in> bar p \<or> Glb a \<in> wrs p)" |
+    "ord (cas\<^sub>F a e\<^sub>1) p = (fence \<in> bar p \<or> Glb a \<in> wrs p \<or> Glb a \<in> rds p)"
+
+subsection \<open>Point Manipulations\<close>
+
+text \<open>Strengthen a point based on a strictly earlier instruction\<close>
+definition stren :: "('v,'r,'a) subbasic \<Rightarrow> ('v,'r,'a) point \<Rightarrow> ('v,'r,'a) point"
+  where
+    "stren a p = p\<lparr> wrs := wrs p \<union> wr (inst a), 
+                    rds := rds p - (wr (inst a) \<inter> locals) \<union> rd (inst a), 
+                    bar := bar p \<union> barriers (inst a) \<rparr>"
+
+text \<open>Weaken a point based on a reorderable instruction\<close>
+definition wken :: "('v,'r,'a) subbasic \<Rightarrow> ('v,'r,'a) point \<Rightarrow> ('v,'r,'a) point"
+  where
+    "wken \<alpha> p = p\<lparr> rds := rds p - wr (inst \<alpha>) \<union> 
+                            (if wr (inst \<alpha>) \<inter> rds p \<noteq> {} then Reg ` deps\<^sub>E (exp (inst \<alpha>)) else {}), 
+                   esc := esc p \<union> wr (inst \<alpha>),
+                   pairs := pairs p \<union> (case inst \<alpha> of cfence \<Rightarrow> {} | _ \<Rightarrow> {(\<alpha>, esc p)}) \<rparr>"
+
+text \<open>Convert an instruction into a point\<close>
+abbreviation gen :: "('v,'r,'a) subbasic \<Rightarrow> ('v,'r,'a) point"
+  where "gen a \<equiv> \<lparr> op = a, wrs = wr (inst a), 
+                   rds = rd (inst a), bar = barriers (inst a), 
+                   esc = {}, pairs = {} \<rparr>"
+
+text \<open>Process a new instruction against one point\<close>
+definition proc1 :: "('v,'r,'a) subbasic \<Rightarrow> (_,_,_) point \<Rightarrow> (_,_,_) points"
+  where "proc1 \<alpha> p \<equiv> if ord (inst \<alpha>) p then {stren \<alpha> p} else {stren \<alpha> p, wken \<alpha> p}"
+
+text \<open>Process a new instruction against a set of points\<close>
+definition rif\<^sub>i :: "('v,'r,'a) subbasic \<Rightarrow> (_,_,_) points \<Rightarrow> (_,_,_) points"
+  where "rif\<^sub>i a P \<equiv> { gen a } \<union> \<Union> (proc1 a ` P)"
+
+text \<open>Process a sequence\<close>
+fun rifseq
+  where
+    "rifseq [] P = P" | 
+    "rifseq (a#t) P = rif\<^sub>i a (rifseq t P)"
+
+text \<open>Process a full program, lifted to low-level choice and loop structures\<close>
+fun rif :: "(('v,'r,'a) auxop, ('v,'r,'a) state) com \<Rightarrow> (_,_,_) points \<Rightarrow> (_,_,_) points"
+  where 
+    "rif (Basic a) P = rif\<^sub>i a P" |
+    "rif (Choice c\<^sub>1 c\<^sub>2) P = (rif c\<^sub>1 P \<union> rif c\<^sub>2 P)" |
+    "rif (SeqChoice s) P = (if s = {} then P else \<Union>((\<lambda>a. rifseq a P) ` s))" |
+    "rif (c\<^sub>1 ;; c\<^sub>2) P = rif c\<^sub>1 (rif c\<^sub>2 P)" |
+    "rif (Ord c\<^sub>1 c\<^sub>2) P = rif c\<^sub>1 (rif c\<^sub>2 P)" |
+    "rif _ P = P"
+
+subsection \<open>Interference Check\<close>
+
+definition escape
+  where "escape V \<alpha> \<equiv> { ((\<beta>,snd (tag \<alpha>)),vc \<alpha>,beh\<^sub>a (\<beta>,snd (tag \<alpha>))) | \<beta>. \<beta> \<in> forall V (inst \<alpha>) }"
+
+definition chk
+  where
+    "chk \<beta> \<alpha> R G \<equiv> \<forall>\<alpha>'. wfbasic \<beta> \<longrightarrow> reorder_inst \<alpha>' \<beta> \<alpha> \<longrightarrow> guar\<^sub>\<alpha> (fwd\<^sub>s \<alpha> (tag \<beta>)) (step G) \<and> 
+                   (\<forall>Q. stabilize R (wp\<^sub>\<alpha> \<beta> (stabilize R (wp\<^sub>\<alpha> \<alpha> (stabilize R Q)))) \<subseteq>
+                        stabilize R (wp\<^sub>\<alpha> \<alpha>' (stabilize R (wp\<^sub>\<alpha> \<beta> (stabilize R Q)))))"
+
+definition chke
+  where
+    "chke \<beta> \<alpha> R G \<equiv> \<forall>\<alpha> \<in> escape (snd \<beta>) \<alpha>. chk (fst \<beta>) \<alpha> R G"
+
+definition checks
+  where "checks P R G \<equiv> \<forall>p \<in> P. \<forall>\<beta> \<in> pairs p. chke \<beta> (op p) R G"
+
+section \<open>Soundness\<close>
+
+subsection \<open>Mono Properties\<close>
+
+text \<open>A series of mono properties to help in reasoning about least-fixed-point\<close>
+
+lemma mono_rif\<^sub>i:
+  "mono (rif\<^sub>i a)"
+  apply (rule monoI)
+  unfolding rif\<^sub>i_def by blast
+
+lemma mono_rifseq:
+  "mono (rifseq a)"
+proof (induct a)
+  case Nil
+  then show ?case by (rule monoI) simp 
+next
+  case (Cons a1 a2)
+  then show ?case by simp (meson monoE monoI mono_rif\<^sub>i)
+qed  
+
+lemma mono_rif:
+  "mono (rif c)"
+proof (induct c)
+  case (Seq c1 c2)
+  then show ?case by (simp add: mono_def)
+next
+  case (Choice c1 c2)
+  then show ?case
+    by (smt Un_mono mono_def rif.simps(2))
+next
+  case (SeqChoice x)
+  then show ?case using mono_rifseq by (simp add: mono_def, intro allI impI SUP_mono') auto
+next
+  case (Ord c1 c2)
+  then show ?case by (simp add: mono_def)
+qed (simp add: monoI mono_rif\<^sub>i)+
+
+lemma mono_union_rif:
+  "mono (\<lambda>Y. P \<union> rif c Y)"
+  by (smt Un_mono monoD monoI mono_rif sup.idem sup.order_iff)
+
+lemma lfp_const:
+  "x \<in> P \<longrightarrow> x \<in> lfp (\<lambda>Y. P \<union> f Y)"
+  by (meson Un_subset_iff basic_trans_rules(31) lfp_greatest)
+
+subsection \<open>Helper Properties\<close>
+
+text \<open>A series of helper properties, generally useful simplifications\<close>
+
+lemma op_proc1 [simp]:
+  "\<forall>q \<in> proc1 x p. op q = op p"
+  by (auto simp: stren_def wken_def proc1_def)
+
+lemma pairs_proc1:
+  "\<forall>q \<in> proc1 x p. pairs q \<supseteq> pairs p"
+  unfolding proc1_def stren_def wken_def by clarsimp
+
+lemma proc1_non_nil [intro]:
+  "proc1 x p \<noteq> {}"
+  unfolding proc1_def stren_def wken_def by clarsimp
+
+lemma [intro]:
+  "stren \<alpha> q \<in> proc1 \<alpha> q"
+  unfolding proc1_def by auto
+
+subsection \<open>Pairwise Check Properties\<close>
+
+text \<open>Properties of the pairwise interference check\<close>
+
+lemma stabilize':
+  "transitive R \<Longrightarrow> stable\<^sub>t R P \<Longrightarrow> P \<subseteq> stabilize R P"
+  unfolding stabilize_def transitive_def stable_def step\<^sub>t_def
+  by auto
+
+lemma stabilize'':
+  "reflexive R \<Longrightarrow> stable\<^sub>t R Q \<Longrightarrow> stabilize R Q = Q"
+  unfolding stabilize_def reflexive_def stable_def step\<^sub>t_def
+  by auto
+
+text \<open>Pairwise check implies the abstract interference freedom property\<close>
+lemma chk_sound:       
+  "wellformed R G \<Longrightarrow> chk \<beta> \<alpha> R G \<Longrightarrow> wfbasic \<beta> \<Longrightarrow> reorder_inst \<alpha>' \<beta> \<alpha> \<Longrightarrow> inter\<^sub>\<alpha> (step\<^sub>t R) (step G) \<beta> \<alpha>"
+proof (clarsimp simp: inter\<^sub>\<alpha>_def, goal_cases)
+  case (1 P M Q)
+  \<comment> \<open>Nominate the strongest-postcondition of \<alpha> from P as the state between \<alpha> and \<beta>\<close>  
+  let ?M="{m. \<exists>m' m''. m' \<in> P \<and> (m',m'') \<in> beh (fwd\<^sub>s \<alpha> (tag \<beta>)) \<and> (m'',m) \<in> step\<^sub>t R}"
+  let ?a="fwd\<^sub>s \<alpha> (tag \<beta>)"
+
+  \<comment> \<open>Establish stability for P, Q and the new intermediate state, in addition to guarantees\<close>
+  have stablePQ: "stable\<^sub>t R P" "stable\<^sub>t R Q" "guar\<^sub>\<alpha> \<alpha> (step G)" "guar\<^sub>\<alpha> \<beta> (step G)"
+    using 1 by (auto simp: atomic_rule_def)
+  have stableM: "stable\<^sub>t R ?M" using 1 unfolding stable_def transitive_def step\<^sub>t_def by force
+
+  \<comment> \<open>Extract order independence properties\<close> 
+  have ref: "\<forall>Q. stabilize R (wp\<^sub>\<alpha> \<beta> (stabilize R (wp\<^sub>\<alpha> \<alpha> (stabilize R Q)))) \<subseteq>
+                 stabilize R (wp\<^sub>\<alpha> ?a (stabilize R (wp\<^sub>\<alpha> \<beta> (stabilize R Q))))"
+    using 1 by (auto simp: chk_def)
+  have g: "guar\<^sub>\<alpha> ((fwd\<^sub>s \<alpha> (tag \<beta>))) (step G)" using 1 by (auto simp: chk_def)
+
+  \<comment> \<open>Show transition from P to Q is independent of order\<close>
+  have p: "P \<subseteq> wp\<^sub>\<alpha> \<beta> M" "M \<subseteq> wp\<^sub>\<alpha> \<alpha> Q" "M \<subseteq> stabilize R M" "P \<subseteq> stabilize R P" "Q \<subseteq> stabilize R Q"
+    using 1 stabilize' unfolding atomic_rule_def by (auto)
+  hence "P \<subseteq> stabilize R (wp\<^sub>\<alpha> \<beta> (stabilize R (wp\<^sub>\<alpha> \<alpha> (stabilize R Q))))" 
+    unfolding wp_def stabilize_def by blast
+  hence exec: "P \<subseteq> stabilize R (wp\<^sub>\<alpha> ?a (stabilize R (wp\<^sub>\<alpha> \<beta> (stabilize R Q))))" 
+    using ref by (auto simp: )
+  hence exec': "P \<subseteq> stabilize R (wp\<^sub>\<alpha> ?a (stabilize R (wp\<^sub>\<alpha> \<beta> (Q))))" 
+    using stabilize'' stablePQ(2) 1 by force
+  hence vc: "P \<subseteq> vc ?a" using 1 by (auto simp: reflexive_def stabilize_def wp_def)
+
+  \<comment> \<open>Establish the late judgement over \<beta>\<close>
+  have "step\<^sub>t R,step G \<turnstile>\<^sub>A ?M {\<beta>} Q" 
+  proof (unfold atomic_rule_def, intro conjI Int_greatest)
+    show "?M \<subseteq> wp\<^sub>\<alpha> \<beta> Q" using exec' 1 
+      unfolding wp_def stabilize_def step\<^sub>t_def reflexive_def transitive_def
+      apply auto
+      by fast
+  qed (insert stablePQ stableM, auto)
+
+  \<comment> \<open>Establish the early judgement over the new \<alpha>\<close>
+  moreover have "step\<^sub>t R,step G \<turnstile>\<^sub>A P {?a} ?M"
+  proof (unfold atomic_rule_def, intro conjI Int_greatest)
+    show "P \<subseteq> wp\<^sub>\<alpha> ?a ?M" using vc 1 unfolding wp_def reflexive_def step\<^sub>t_def by auto
+  qed (insert stablePQ stableM g, auto)
+
+  ultimately show ?case by blast
+qed
+
+
+
+fun exec
+  where 
+    "exec m (subop.op x e) = (m (Reg x :=\<^sub>s ev\<^sub>E (rg m) e))" | 
+    "exec m (subop.cstore b x e) = (m (Glb x :=\<^sub>s ev\<^sub>E (rg m) e))" | 
+    "exec m (subop.cas\<^sub>T x e\<^sub>1 e\<^sub>2) = (m (Glb x :=\<^sub>s ev\<^sub>E (rg m) e\<^sub>2))" | 
+    "exec m _ = m"
+
+lemma beh_fwd\<^sub>i [simp]:
+  "beh\<^sub>i (fwd\<^sub>i \<alpha> \<beta>) = {(m\<^sub>1,upd (wr \<alpha>) (st m) m\<^sub>1) | m m\<^sub>1. (exec m\<^sub>1 \<beta>,m) \<in> beh\<^sub>i \<alpha>}"
+  apply (cases \<beta>; auto)
+  apply (cases \<alpha>; clarsimp split: if_splits)
+  apply (cases \<alpha>; clarsimp split: if_splits)
+  apply (cases \<alpha>; clarsimp split: if_splits)
+  apply (cases \<alpha>; clarsimp split: if_splits)
+  apply (cases \<alpha>; clarsimp split: if_splits)
+  apply (cases \<alpha>; clarsimp split: if_splits)+
+  done
+
+lemma [simp]:
+  "upd (dom (\<lambda>y. if x = y then Some c else M y)) (the \<circ> (\<lambda>y. if x = y then Some c else M y)) m = 
+  (upd (dom M) (the o M) m)(x :=\<^sub>s c)"
+  apply (auto simp: upd_def st_upd_def intro!: state_rec.equality)
+  by force
+
+lemma escE:
+  assumes "\<beta> \<in> escape V \<alpha>"
+  obtains M where "V = dom M" "vc \<beta> = vc \<alpha>" "beh \<beta> = beh\<^sub>a (smap (inst \<alpha>) M,snd (tag \<alpha>))" "snd (tag \<beta>) = snd (tag \<alpha>)" "inst \<beta> = smap (inst \<alpha>) M" 
+  using assms unfolding escape_def forall_def by auto   
+
+lemma ev_upd_exec [simp]:
+  "wfbasic \<gamma> \<Longrightarrow> (m,m') \<in> beh \<gamma> \<Longrightarrow> ev\<^sub>E (rg (upd V f (exec m (inst \<gamma>)))) e = ev\<^sub>E (rg (upd V f m')) e"
+  apply (rule deps_ev\<^sub>E)
+  apply simp
+  apply (cases \<gamma> rule: opbasicE) 
+  by (auto simp: wfbasic_def)
+
+lemma vc_fwd\<^sub>s[simp]:
+  "vc (fwd\<^sub>s \<alpha> \<beta>) = vc \<alpha>"
+  by (cases \<alpha> rule: opbasicE; cases \<beta>; case_tac a; auto simp: Let_def split: if_splits)
+
+lemma beh_fwd\<^sub>s [simp]:
+  "beh (fwd\<^sub>s \<alpha> \<beta>) = ( beh\<^sub>a (fwd\<^sub>i (inst \<alpha>) (fst \<beta>), (snd (tag \<alpha>))) )"
+  by (cases \<alpha> rule: opbasicE; cases \<beta>; case_tac a; auto simp: wfbasic_def Let_def split: if_splits)
+
+lemma [simp]:
+  "wr \<beta> = {x} \<Longrightarrow> inst (fwd\<^sub>s \<alpha> (\<beta>, f)) = (subst\<^sub>i (inst \<alpha>) x (exp \<beta>))"
+  by (cases \<beta>; cases \<alpha>) auto
+
+lemma aux_fwd\<^sub>s [simp]:
+  "snd (tag (fwd\<^sub>s \<alpha> \<beta>)) = snd (tag \<alpha>)"
+  by (cases \<alpha> rule: opbasicE; cases \<beta>; case_tac a; auto simp: Let_def split: if_splits)
+
+lemma [simp]:
+  "wr (inst (fwd\<^sub>s \<alpha> ( \<beta>))) = wr (inst \<alpha>)"
+  by (cases \<alpha> rule: opbasicE; cases \<beta>; case_tac a; auto simp: Let_def split: if_splits)
+
+lemma escape_guar:
+  assumes "wr \<beta> = {x}" 
+  assumes "\<forall>\<alpha>' \<in> escape (insert x V) \<alpha>. guar\<^sub>\<alpha> (fwd\<^sub>s \<alpha>' \<gamma>) (step G)"
+  shows "\<forall>\<alpha>' \<in> escape V (fwd\<^sub>s \<alpha> (\<beta>,f)). guar\<^sub>\<alpha> (fwd\<^sub>s \<alpha>' \<gamma>) (step G)"
+  unfolding guar_def
+proof (auto split: subop.splits elim!: escE, goal_cases)
+  case (1 M m\<^sub>1 m\<^sub>2)
+  let ?m = "exec m\<^sub>1 (fst \<gamma>)"
+  let ?M = "\<lambda>y. (if x = y then Some (ev\<^sub>E (rg (upd (dom M) (the \<circ> M) ?m)) (exp \<beta>)) else M y)"
+  let ?i = "smap (inst \<alpha>) ?M"
+  let ?\<alpha> = "((?i, snd (tag \<alpha>)), vc \<alpha>, beh\<^sub>a (?i, snd (tag \<alpha>)))"
+
+  have "insert x V = dom ?M" using 1 by auto
+  hence "?\<alpha> \<in> escape (insert x V) \<alpha>" unfolding escape_def by auto
+  moreover have "m\<^sub>1 \<in> vc (fwd\<^sub>s ?\<alpha> \<gamma>)" using 1 by auto
+  moreover have "(m\<^sub>1, (upd (wr (inst \<alpha>)) (st m\<^sub>2) m\<^sub>1)(aux: snd (tag \<alpha>))) \<in> beh (fwd\<^sub>s ?\<alpha> \<gamma>)"
+    using 1 assms(1,2)
+    apply (clarsimp, intro exI conjI)
+      prefer 2
+    by simp+
+
+  ultimately show ?case using assms unfolding guar_def by blast
+qed
+
+lemma escape_wp:
+  assumes "wfbasic \<gamma>" "wr \<beta> = {x}"
+  assumes "\<forall>\<alpha>' \<in> escape (insert x V) \<alpha>. stabilize R (wp\<^sub>\<alpha> \<gamma> (stabilize R (wp\<^sub>\<alpha> \<alpha>' (stabilize R Q)))) \<subseteq>
+                                      stabilize R (wp\<^sub>\<alpha> (fwd\<^sub>s \<alpha>' (tag \<gamma>)) (stabilize R (wp\<^sub>\<alpha> \<gamma> (stabilize R Q))))"
+  shows "\<forall> \<alpha>' \<in> escape V (fwd\<^sub>s \<alpha> (\<beta>,f)). 
+    \<forall>\<alpha>''. reorder_inst \<alpha>'' \<gamma> \<alpha>' \<longrightarrow> stabilize R (wp\<^sub>\<alpha> \<gamma> (stabilize R (wp\<^sub>\<alpha> \<alpha>' (stabilize R Q)))) \<subseteq>
+                              stabilize R (wp\<^sub>\<alpha> (fwd\<^sub>s \<alpha>' (tag \<gamma>)) (stabilize R (wp\<^sub>\<alpha> \<gamma> (stabilize R Q))))" 
+proof (intro allI impI ballI subsetI, elim escE, goal_cases)
+  case (1 \<alpha>' \<alpha>'' m M)
+  let ?m = "exec m (inst \<gamma>)"
+  let ?M = "\<lambda>y. (if x = y then Some (ev\<^sub>E (rg (upd (dom M) (the \<circ> M) ?m)) (exp \<beta>)) else M y)"
+  let ?i = "smap (inst \<alpha>) ?M"
+  let ?\<alpha> = "((?i, snd (tag \<alpha>)), vc \<alpha>, beh\<^sub>a (?i, snd (tag \<alpha>)))"
+
+  have "insert x V = dom ?M" using 1 by auto
+  hence esc: "?\<alpha> \<in> escape (insert x V) \<alpha>" unfolding escape_def by auto
+
+  have e: "\<forall>m'. rg m = rg m' \<longrightarrow> 
+      ev\<^sub>E (rg (upd (dom M) (the \<circ> M) (exec m (inst \<gamma>)))) (exp \<beta>) =
+      ev\<^sub>E (rg (upd (dom M) (the \<circ> M) (exec m' (inst \<gamma>)))) (exp \<beta>)"
+    by (intro allI impI ballI deps_ev\<^sub>E) (cases "inst \<gamma>"; simp)
+
+  have "m \<in> stabilize R (wp\<^sub>\<alpha> \<gamma> (stabilize R (wp\<^sub>\<alpha> ?\<alpha> (stabilize R Q))))"
+    using 1 assms(2)
+    unfolding stabilize_def wp_def
+    apply auto
+    apply (rename_tac m\<^sub>1 m\<^sub>2 m\<^sub>4 m\<^sub>3 m\<^sub>5)
+    apply (subgoal_tac "ev\<^sub>E (rg (upd (dom M) (the \<circ> M) ?m)) (exp \<beta>) = ev\<^sub>E (rg (upd (dom M) (the \<circ> M) m\<^sub>3)) (exp \<beta>)")
+    apply fastforce
+    apply (subgoal_tac "ev\<^sub>E (rg (upd (dom M) (the \<circ> M) m\<^sub>2)) (exp \<beta>) = ev\<^sub>E (rg (upd (dom M) (the \<circ> M) m\<^sub>3)) (exp \<beta>)")
+    apply (subgoal_tac "ev\<^sub>E (rg (upd (dom M) (the \<circ> M) (exec m\<^sub>1 (inst \<gamma>)))) (exp \<beta>) = ev\<^sub>E (rg (upd (dom M) (the \<circ> M) m\<^sub>2)) (exp \<beta>)")
+    using e assms(1) apply force
+    using assms(1) apply auto[1]
+    by (rule deps_ev\<^sub>E) (auto)
+
+  hence "m \<in> stabilize R (wp\<^sub>\<alpha> (fwd\<^sub>s ?\<alpha> (tag \<gamma>)) (stabilize R (wp\<^sub>\<alpha> \<gamma> (stabilize R Q))))"
+    using assms(3) 1 esc by blast
+  thus ?case using 1(4,5,6,7) assms(2)
+    unfolding stabilize_def wp_def 
+    apply auto
+     apply (clarsimp simp add: e)
+    apply fastforce
+    apply (clarsimp simp add: e)
+    by fastforce
+qed
+
+lemma [simp]:
+  "wr (subst\<^sub>g \<alpha> x22 x23) = wr \<alpha>"
+  by (cases \<alpha>; auto)
+
+lemma substg_rd [simp]:
+  "rd (subst\<^sub>g \<alpha> x e) = rd \<alpha> - {Glb x} \<union> (if Glb x \<in> rd \<alpha> then Reg ` deps\<^sub>E e else {})"
+  by (cases \<alpha>; auto)
+
+lemma substr_rd [simp]:
+  "rd (subst\<^sub>r \<alpha> x e) = rd \<alpha> - {Reg x} \<union> (if Reg x \<in> rd \<alpha> then Reg ` deps\<^sub>E e else {})"
+  by (cases \<alpha>; auto)
+
+lemma substr_wr [simp]:
+  "wr (subst\<^sub>r \<alpha> x e) = wr \<alpha>"
+  by (cases \<alpha>; auto)
+
+lemma [simp]:
+  "barriers \<alpha> = {fence} \<Longrightarrow> \<alpha> = fence"
+  "barriers \<alpha> = {stfence} \<Longrightarrow> \<alpha> = stfence"
+  "barriers \<alpha> = {cfence} \<Longrightarrow> \<alpha> = cfence"
+  by (cases \<alpha>; auto)+
+
+lemma reorder_imp:
+  assumes "re\<^sub>i \<beta> \<alpha>"
+  assumes "barriers \<alpha> = barriers \<alpha>'"
+  assumes "wr \<alpha> = wr \<alpha>'"
+  assumes "rd \<alpha>' \<subseteq> rd \<alpha>"
+  shows "re\<^sub>i \<beta> \<alpha>'"
+  using assms
+  apply (cases \<beta>; clarsimp)
+  by (intro conjI; clarsimp; blast)+
+
+lemma fwd_barriers [simp]:
+  "barriers (fwd\<^sub>i \<alpha> \<beta>) = barriers \<alpha>"
+  by (cases \<alpha>; cases \<beta>; auto)
+
+lemma escape_barriers [simp]:
+  "\<forall>\<alpha> \<in> escape V \<beta>. barriers (inst \<alpha>) = barriers (inst \<beta>)"
+  unfolding escape_def by auto
+
+lemma [simp]:
+  "inst (fwd\<^sub>s \<alpha> \<beta>) = fwd\<^sub>i (inst \<alpha>) (fst \<beta>)"
+  by (cases \<beta>; cases \<alpha>; auto)
+
+lemma fwd_wr [simp]:
+  "wr (fwd\<^sub>i \<alpha> \<beta>) = wr \<alpha>"
+  by (cases \<alpha>; cases \<beta>; auto)
+
+lemma escape_wr [simp]:
+  "\<forall>\<alpha> \<in> escape V \<beta>. wr (inst \<alpha>) = wr (inst \<beta>)"
+  unfolding escape_def by auto
+
+lemma fwd_rd [simp]:
+  "rd (fwd\<^sub>i \<alpha> \<beta>) = (if wr \<beta> \<inter> rd \<alpha> \<noteq> {} then rd \<alpha> - wr \<beta> \<union>  Reg ` deps\<^sub>E (exp \<beta>) else rd \<alpha>)"
+  by (cases \<alpha>; cases \<beta>; auto)
+
+lemma escape_rd [simp]:
+  "\<forall>\<alpha> \<in> escape V \<beta>. rd (inst \<alpha>) = rd (inst \<beta>) - V"
+  unfolding escape_def by auto
+
+lemma escape_reorder:
+  assumes "\<alpha>' \<in> escape V (fwd\<^sub>s \<alpha> \<beta>)" "reorder_inst \<alpha>'' \<gamma> \<alpha>'"
+  shows "\<forall>\<alpha>'\<in>escape (wr (fst \<beta>) \<union> V) \<alpha>. \<exists>\<alpha>''. reorder_inst \<alpha>'' \<gamma> \<alpha>'"
+  using assms
+proof (intro ballI, goal_cases)
+  case (1 \<alpha>'')
+  hence a: "re\<^sub>i (inst \<gamma>) (fwd\<^sub>i (inst \<alpha>') (inst \<gamma>))"
+    by (cases \<gamma>, cases \<alpha>', clarsimp)
+  hence "re\<^sub>i (inst \<gamma>) (fwd\<^sub>i (inst \<alpha>'') (inst \<gamma>))"
+    apply (rule reorder_imp) 
+    using 1 by auto
+  then show ?case by (cases \<gamma>, cases \<alpha>'', clarsimp)
+qed
+
+lemma escape_check:
+  assumes "wr \<beta> = {x}"
+  assumes "\<forall>\<alpha>' \<in> escape (wr \<beta> \<union> V) \<alpha>. chk \<gamma> \<alpha>' R G"
+  shows "\<forall>\<alpha>' \<in> escape V (fwd\<^sub>s \<alpha> (\<beta>,f)). chk \<gamma> \<alpha>' R G"
+  unfolding chk_def
+proof (intro ballI allI impI conjI, goal_cases)
+  case (1 \<alpha>' \<alpha>'')
+  hence "\<forall>\<alpha>' \<in> escape (wr \<beta> \<union> V) \<alpha>. guar\<^sub>\<alpha> (fwd\<^sub>s \<alpha>' (tag \<gamma>)) (step G)"
+    using assms(2) escape_reorder[OF 1(1)] by (auto simp: chk_def)
+  then show ?case using escape_guar[OF assms(1), of V \<alpha> "tag \<gamma>"] 1 unfolding assms(1) by simp
+next
+  case (2 \<alpha>' \<alpha>'' Q)
+  hence "\<forall>\<alpha>' \<in> escape (wr \<beta> \<union> V) \<alpha>. stabilize R (wp\<^sub>\<alpha> \<gamma> (stabilize R (wp\<^sub>\<alpha> \<alpha>' (stabilize R Q)))) \<subseteq>
+      stabilize R (wp\<^sub>\<alpha> (fwd\<^sub>s \<alpha>' (tag \<gamma>)) (stabilize R (wp\<^sub>\<alpha> \<gamma> (stabilize R Q))))"
+    using assms(2) escape_reorder[OF 2(1)] by (auto simp: chk_def)
+  then show ?case using escape_wp[OF 2(2) assms(1), of V] 2 assms unfolding assms(1) by simp
+qed
+
+text \<open>
+Given two reorderable instructions, escaping the writes of the earlier instruction
+implies a check over the forwarded variant.
+\<close>
+lemma chke_sound:
+  assumes "reorder_inst \<alpha>' \<beta> \<alpha>" "wfbasic \<beta>" "wfbasic \<alpha>"
+  assumes "chke (\<gamma>, wr (inst \<beta>) \<union> V) \<alpha> R G" 
+  shows "chke (\<gamma>, V) \<alpha>' R G"
+  unfolding chke_def
+proof (intro ballI allI impI, simp)
+  fix \<alpha>'' assume e: "\<alpha>'' \<in> escape V \<alpha>'"
+  show "chk \<gamma> \<alpha>'' R G" using assms(1)
+  proof (cases rule: fwdE)
+    case no_fwd
+    hence "forall V (inst \<alpha>') = forall (wr (inst \<beta>) \<union> V) (inst \<alpha>)"
+      by (cases "inst \<beta>") fastforce+
+    hence "escape V \<alpha>' = escape (wr (inst \<beta>) \<union> V) \<alpha>"
+      using no_fwd unfolding escape_def by simp
+    thus ?thesis using e assms(4) unfolding chke_def by auto
+  next
+    case (fwd x)
+    thus ?thesis using fwd escape_check[of "inst \<beta>" x V \<alpha>] e assms(1,4) 
+      unfolding chke_def by (cases "tag \<beta>") simp
+  qed
+qed
+
+text \<open>Escape check with an empty escape set implies a full check\<close>
+lemma chke_nil_esc:
+  assumes "chke (\<beta>, {}) \<alpha> R G" "wfbasic \<alpha>"
+  shows "chk \<beta> \<alpha> R G"
+proof -
+  have "\<alpha> \<in> escape {} \<alpha>" using assms(2) by (cases \<alpha>; auto simp: wfbasic_def escape_def) 
+  thus "chk \<beta> \<alpha> R G" using assms by (auto simp:  chke_def)
+qed
+
+text \<open>\<close>
+lemma inter_cfence:
+  assumes "inst \<beta> = cfence" "wfbasic \<beta>" "wfbasic \<alpha>" "reorder_inst \<alpha>' \<beta> \<alpha>" "wellformed R G"
+  shows "inter\<^sub>\<alpha> (step\<^sub>t R) (step G) \<beta> \<alpha>"
+proof (clarsimp simp: inter\<^sub>\<alpha>_def, goal_cases)
+  case (1 P M Q)
+  \<comment> \<open>Nominate the strongest-postcondition of \<alpha> from P as the state between \<alpha> and \<beta>\<close>  
+  let ?M="{m. \<exists>m' m''. m' \<in> P \<and> (m',m'') \<in> beh (fwd\<^sub>s \<alpha> (tag \<beta>)) \<and> (m'',m) \<in> step\<^sub>t R}"
+  let ?a="fwd\<^sub>s \<alpha> (tag \<beta>)"
+
+  \<comment> \<open>Establish stability for P, Q and the new intermediate state, in addition to guarantees\<close>
+  have stablePQ: "stable\<^sub>t R P" "stable\<^sub>t R Q" "guar\<^sub>\<alpha> \<alpha> (step G)" "guar\<^sub>\<alpha> \<beta> (step G)"
+    using 1 by (auto simp: atomic_rule_def)
+  have stableM: "stable\<^sub>t R ?M" using 1 assms unfolding stable_def transitive_def step\<^sub>t_def by force
+
+  have \<beta>: "beh \<beta> = {(m,m'). m = m'}" "vc \<beta> = UNIV"
+    using assms(1,2) unfolding wfbasic_def by auto
+  have [simp]: "fwd\<^sub>s \<alpha> (tag \<beta>) = \<alpha>"
+    using assms(1,3) 
+    by (cases \<alpha> rule: opbasicE; cases "tag \<beta>"; clarsimp simp: wfbasic_def)
+
+  \<comment> \<open>Show transition from P to Q is independent of order\<close>
+  have p: "P \<subseteq> wp\<^sub>\<alpha> \<beta> M" "M \<subseteq> wp\<^sub>\<alpha> \<alpha> Q" "M \<subseteq> stabilize R M" "P \<subseteq> stabilize R P" "Q \<subseteq> stabilize R Q"
+    using 1 assms stabilize' unfolding atomic_rule_def by (auto)
+  hence "P \<subseteq> stabilize R (wp\<^sub>\<alpha> \<beta> (stabilize R (wp\<^sub>\<alpha> \<alpha> (stabilize R Q))))" 
+    unfolding wp_def stabilize_def by blast
+
+  \<comment> \<open>Establish the late judgement over \<beta>\<close>
+  have "step\<^sub>t R,step G \<turnstile>\<^sub>A Q {\<beta>} Q"
+  proof (unfold atomic_rule_def, intro conjI Int_greatest)
+    show "Q \<subseteq> wp\<^sub>\<alpha> \<beta> Q" by (auto simp: wp_def \<beta>)
+  qed (insert stablePQ stableM, auto)
+
+  \<comment> \<open>Establish the early judgement over the new \<alpha>\<close>
+  moreover have "step\<^sub>t R,step G \<turnstile>\<^sub>A P {?a} Q"
+  proof (unfold atomic_rule_def, intro conjI Int_greatest)
+    show "P \<subseteq> wp\<^sub>\<alpha> ?a Q" using p by (auto simp: wp_def \<beta>)
+  qed (insert stablePQ stableM, auto)
+
+  ultimately show ?case by blast
+qed  
+
+subsection \<open>Silent rif Checks\<close>
+
+lemma [simp]:
+  "rif (seq2com s) P = rifseq s P"
+  by (induct s, auto)
+
+text \<open>Trivial proof showing rif is preserved across silent steps\<close>
+lemma silent_rif_checks:
+  assumes "c \<leadsto> c'" "sim c"
+  shows "rif c' P \<subseteq> rif c P"
+  using assms
+proof (induct arbitrary: P)
+  case (seq2 c\<^sub>2 c\<^sub>2' c\<^sub>1)
+  then show ?case by (simp add: monoD mono_rif)
+qed auto
+
+subsection \<open>Execution rif Checks\<close>
+
+text \<open>The ord test shouldn't establish dependencies between reorderable operations\<close>
+lemma ord_sound [intro]:
+  assumes "reorder_inst \<alpha>' \<beta> \<alpha>"
+  shows "\<not> ord (inst \<beta>) (gen \<alpha>)"
+  using assms 
+  apply (cases \<alpha> rule: opbasicE; cases \<beta> rule: opbasicE) 
+  apply (clarsimp simp: hasGlobal_def)+
+  done
+
+text \<open>
+Show that the checks produced by an instruction \<alpha> with a prefix r are sufficient
+to establish the desired abstract rif properties.
+\<close>
+
+text \<open>
+Relate two points such that their reordering constraints are the same,
+but the checks of one implies the checks of the other, including all future checks.
+\<close>
+definition point_ord (infix "\<prec>" 60)
+  where "point_ord p q \<equiv>  
+            wrs p = wrs q \<and> rds p = rds q \<and> (bar p = bar q) \<and> 
+            (\<forall>R G (\<alpha> :: ('v,'r,'a) subbasic) V. 
+              chke (\<alpha>, esc p \<union> V) (op p) R G \<longrightarrow> chke (\<alpha>, esc q \<union> V) (op q) R G) \<and>
+            (\<forall>R G. (\<forall>\<beta> \<in> pairs p. chke \<beta> (op p) R G) \<longrightarrow> (\<forall>\<beta> \<in> pairs q. chke \<beta> (op q) R G))"
+
+text \<open>
+Extend this point relation over two sets of points, such that for all points in the RHS,
+one exists in the LHS that establishes the relation.
+\<close>
+definition points_ord (infix "\<prec>\<prec>" 60)
+  where "points_ord P Q \<equiv> \<forall>q \<in> Q. \<exists>p \<in> P. p \<prec> q"
+
+text \<open>The point relation is reflexive\<close>
+lemma point_ord_refl [intro]:
+  "p \<prec> p" 
+  by (auto simp: point_ord_def)
+
+text \<open>The point relation is preserved across stren\<close>
+lemma point_ord_stren [intro]:
+  "p \<prec> q \<Longrightarrow> stren \<alpha> p \<prec> stren \<alpha> q"
+  by (auto simp: point_ord_def stren_def)
+
+text \<open>The point relation is preserved across wken\<close>
+lemma point_ord_wken [intro]:
+  "p \<prec> q \<Longrightarrow> wken \<alpha> p \<prec> wken \<alpha> q"
+  unfolding point_ord_def wken_def
+  apply (auto simp: Un_assoc sup_assoc split: subop.splits)
+  by (cases \<alpha>; case_tac a; metis sup_bot_right)+
+
+text \<open>The point relation ensures equivalent ordering constraints\<close>
+lemma point_ord [simp]:
+  "p \<prec> q \<Longrightarrow> ord \<alpha> p = ord \<alpha> q"
+  by (cases \<alpha>) (clarsimp simp: point_ord_def)+
+
+text \<open>Based on the above, proc1 preserves the point relation\<close>
+lemma point_ord_proc1 [intro]:
+  "p \<prec> q \<Longrightarrow> proc1 \<alpha> p \<prec>\<prec> proc1 \<alpha> q"
+  unfolding points_ord_def proc1_def by auto
+
+text \<open>Based on the above, proci preserves the point relation\<close>
+lemma points_ord_rif\<^sub>i [intro]:
+  "P \<prec>\<prec> Q \<Longrightarrow> rif\<^sub>i \<alpha> P \<prec>\<prec> rif\<^sub>i \<alpha> Q"
+  using point_ord_proc1 unfolding rif\<^sub>i_def points_ord_def by fast
+
+lemma points_ord_rifseq [intro]:
+  "P \<prec>\<prec> Q \<Longrightarrow> rifseq a P \<prec>\<prec> rifseq a Q"
+  by (induct a, auto)
+
+lemma points_ord_union [intro]:
+  "P \<prec>\<prec> Q \<Longrightarrow> P' \<prec>\<prec> Q' \<Longrightarrow> P \<union> P' \<prec>\<prec> Q \<union> Q'"
+  by (auto simp: points_ord_def)
+
+text \<open>Finally, rif preserves the point relation\<close>
+lemma points_ord_rif [intro]:
+  "P \<prec>\<prec> Q \<Longrightarrow> rif c P \<prec>\<prec> rif c Q"
+proof (induct c arbitrary: P Q)
+  case (SeqChoice x)
+  then show ?case using points_ord_rifseq[OF SeqChoice] 
+    by (auto simp: points_ord_def) blast
+qed auto
+
+lemma [simp]:
+  "wr (inst (fwd\<^sub>s \<alpha> (tag \<beta>))) = wr (inst \<alpha>)"
+  by (cases \<alpha> rule: opbasicE; cases \<beta> rule: opbasicE; auto simp: Let_def split: if_splits)
+
+lemma [simp]:
+  "barriers (inst (fwd\<^sub>s \<alpha> (tag \<beta>))) = barriers (inst \<alpha>)"
+  by (cases \<alpha> rule: opbasicE; cases \<beta> rule: opbasicE; auto simp: Let_def split: if_splits)
+
+lemma [simp]:
+  "rd (inst (fwd\<^sub>s \<alpha> (tag \<beta>))) = 
+    (if wr (inst \<beta>) \<inter> rd (inst \<alpha>) \<noteq> {} then rd (inst \<alpha>) - wr (inst \<beta>) \<union>  Reg ` deps\<^sub>E (exp (inst \<beta>)) 
+    else rd (inst \<alpha>))"
+  by (cases \<alpha> rule: opbasicE; cases \<beta> rule: opbasicE; auto)
+
+text \<open>Establish the point relation between \<alpha> weakened by \<beta> and one generated from \<alpha>' directly\<close>
+lemma point_ord_fwd:
+  assumes "reorder_inst \<alpha>' \<beta> \<alpha>" "wfbasic \<beta>" "wfbasic \<alpha>"
+  shows "wken \<beta> (gen \<alpha>) \<prec> gen \<alpha>'"
+  using assms apply (auto simp: point_ord_def wken_def)
+  by (insert chke_sound, blast)+
+
+text \<open>Checks against the LHS of a points relation imply checks against the RHS\<close>
+lemma points_ord_checks [intro]:
+  "checks P R G \<Longrightarrow> P \<prec>\<prec> Q \<Longrightarrow> checks Q R G"
+  unfolding checks_def points_ord_def point_ord_def by metis
+
+lemma rifseq_checks_postfix [intro]:
+  assumes "checks (rifseq a P) R G"
+  shows "checks P R G"
+  using assms
+proof (induct a arbitrary: P)
+  case Nil
+  then show ?case by auto
+next
+  case (Cons a1 a2)
+  hence "checks (rifseq a2 P) R G" unfolding checks_def
+  proof (intro ballI)
+    fix p \<beta> assume a: "p \<in> rifseq a2 P" "\<beta> \<in> pairs p"
+    hence "\<exists>q \<in> proc1 a1 p. \<beta> \<in> pairs q" using pairs_proc1 proc1_non_nil by blast
+    thus "chke \<beta> (op p) R G"
+      using Cons a by (auto simp: checks_def rif_def rif\<^sub>i_def)
+  qed
+  thus ?case using Cons by auto
+qed
+
+text \<open>rif checks on sequential composition should imply rif checks of just the postfix\<close>
+lemma rif_checks_postfix [intro]:
+  assumes "checks (rif (c ;; r) P) R G"
+  shows "checks (rif r P) R G"
+  using assms
+proof (induct c arbitrary: r P)
+  case (Basic x)
+  show ?case unfolding checks_def
+  proof (intro ballI)
+    fix p \<beta> assume a: "p \<in> rif r P" "\<beta> \<in> pairs p"
+    hence "\<exists>q \<in> proc1 x p. \<beta> \<in> pairs q" using pairs_proc1 proc1_non_nil by blast
+    thus "chke \<beta> (op p) R G"
+      using Basic a by (auto simp: checks_def rif_def rif\<^sub>i_def)
+  qed
+next
+  case (Loop c)
+  thus ?case by (simp add: lfp_const checks_def) 
+next
+  case (SeqChoice x)
+  then show ?case using rifseq_checks_postfix
+    unfolding checks_def by (simp split: if_splits) fastforce
+qed (unfold checks_def rif.simps; blast)+
+
+text \<open>rif checks on sequential composition should imply rif checks of just the prefix\<close>
+lemma rif_checks_prefix [intro]:
+  assumes "checks (rif (c ;; r) P) R G"
+  shows "checks (rif c {}) R G"
+  using assms
+proof -
+  have "rif c {} \<subseteq> rif c (rif r P)" by (simp add: monoD mono_rif)
+  thus ?thesis using assms unfolding checks_def by auto
+qed
+
+text \<open>
+rif checks on sequential composition due to an action that can reorder with the postfix
+correspond to the checks that would be seen if the postfix wasn't present and forwarding
+was captured fully.
+\<close>
+lemma rif_checks_fwd:
+  assumes "reorder_com \<alpha>' c\<^sub>2 \<alpha>" "wfcom c\<^sub>2" "wfbasic \<alpha>" "sim c\<^sub>2"
+  assumes "checks (rif (c\<^sub>1 ;; c\<^sub>2 ;; Basic \<alpha>) {}) R G" 
+  shows "checks (rif (c\<^sub>1 ;; Basic \<alpha>') {}) R G"
+  using assms
+proof (induct \<alpha>' c\<^sub>2 \<alpha> arbitrary: c\<^sub>1 rule: reorder_com.induct)
+  case (2 \<alpha>' \<beta> \<alpha>)
+  text \<open>Remove the checks on gen \<beta>\<close>
+  hence "checks (rif c\<^sub>1 ({gen \<beta>} \<union> proc1 \<beta> (gen \<alpha>))) R G"
+    by (auto simp: rif\<^sub>i_def)
+  hence c: "checks (rif c\<^sub>1 (proc1 \<beta> (gen \<alpha>))) R G"
+    unfolding checks_def using mono_Un mono_rif by blast
+  text \<open>Show the point relation between \<alpha> and \<alpha>'\<close>
+  have r: "reorder_inst \<alpha>' \<beta> \<alpha>" using 2 by auto
+  have "proc1 \<beta> (gen \<alpha>) \<prec>\<prec> {gen \<alpha>'}" 
+    using point_ord_fwd[OF r] ord_sound[OF r] 2(2,3) 
+    unfolding points_ord_def proc1_def wfcom_def by auto
+  text \<open>Use properties of the point relation to establish checks on c1 and \<alpha>'\<close>
+  hence "rif c\<^sub>1 (proc1 \<beta> (gen \<alpha>)) \<prec>\<prec> rif c\<^sub>1 {gen \<alpha>'}" by auto
+  hence "checks (rif c\<^sub>1 {gen \<alpha>'}) R G" using c by blast
+  then show ?case by (auto simp: rif\<^sub>i_def)
+next
+  case (3 \<alpha>' c\<^sub>1' c\<^sub>2 \<alpha>)
+  then obtain \<alpha>'' where \<alpha>: "reorder_com \<alpha>' c\<^sub>1' \<alpha>''" "reorder_com \<alpha>'' c\<^sub>2 \<alpha>" by auto
+  hence "checks (rif (c\<^sub>1 ;; c\<^sub>1' ;; Basic \<alpha>'') {}) R G" 
+    using 3(2)[of _ "c\<^sub>1 ;; c\<^sub>1'"] 3(4,5,6,7) by (auto simp: wfcom_def)
+  moreover have "wfbasic \<alpha>''" using 3 \<alpha> fwd_wfbasic by blast
+  ultimately show ?case using \<alpha> 3 by auto
+next
+  case (4 \<alpha>' c\<^sub>1' c\<^sub>2 \<alpha>)
+  then obtain \<alpha>'' where \<alpha>: "reorder_com \<alpha>' c\<^sub>1' \<alpha>''" "reorder_com \<alpha>'' c\<^sub>2 \<alpha>" by auto
+  hence "checks (rif (c\<^sub>1 ;; c\<^sub>1' ;; Basic \<alpha>'') {}) R G" 
+    using 4(2)[of _ "c\<^sub>1 ;; c\<^sub>1'"] 4(4,5,6,7) by (auto simp: wfcom_def)
+  moreover have "wfbasic \<alpha>''" using 4 \<alpha> fwd_wfbasic by blast
+  ultimately show ?case using \<alpha> 4 by auto
+qed auto 
+
+text \<open>Convert an execution step to a reordering\<close>
+lemma exec_to_reorder:
+  assumes "lexecute c r \<alpha> c'"
+  shows "\<exists>\<alpha>'. reorder_com \<alpha>' r \<alpha>"
+  using assms
+  by (induct, unfold reorder_com.simps(1); blast)
+
+text \<open>Phrase the desired property for induction over a reordering\<close>
+lemma exec_checks_induct:
+  assumes "wellformed R G" "wfcom r" "wfbasic \<alpha>" "sim r"
+  assumes "reorder_com \<alpha>' r \<alpha>"
+  assumes "checks (rif (r ;; Basic \<alpha>) {}) R G"
+  shows "inter\<^sub>c (step\<^sub>t R) (step G) r \<alpha>"
+  using assms
+proof (induct \<alpha>' r \<alpha> rule: reorder_com.induct)
+  case (2 \<alpha>' \<beta> \<alpha>)
+  hence r: "reorder_inst \<alpha>' \<beta> \<alpha>" "wfbasic \<beta>" by (auto simp: wfcom_def)
+  text \<open>Given the two instructions can reorder, they mustn't be considered ordered\<close>
+  hence "\<not> ord (inst \<beta>) (gen \<alpha>)" using ord_sound[of \<alpha>' \<alpha> \<beta>] by auto
+  text \<open>Obtain the point generated for \<alpha>\<close>
+  then obtain p where "p \<in> rif\<^sub>i \<beta> (rif\<^sub>i \<alpha> {})" "op p = \<alpha>" "(\<beta>,{}) \<in> pairs p \<or> inst \<beta> = cfence"
+    unfolding rif\<^sub>i_def proc1_def stren_def wken_def
+    apply (clarsimp split: if_splits subop.splits)
+    by (cases "inst \<beta>"; fastforce)
+  text \<open>Extract the check between \<beta> and \<alpha> and show it establishes inter\<close>
+  hence "chke (\<beta>,{}) \<alpha> R G \<or> inst \<beta> = cfence" using 2(6) by (auto simp: checks_def)
+  thus ?case using chk_sound chke_nil_esc 2(1,3) r inter_cfence  unfolding inter\<^sub>c.simps by blast
+next
+  case (3 \<alpha>' c\<^sub>1 c\<^sub>2 \<alpha>)
+  then obtain \<alpha>'' where \<alpha>: "reorder_com \<alpha>' c\<^sub>1 \<alpha>''" "reorder_com \<alpha>'' c\<^sub>2 \<alpha>" by auto
+  hence w:  "wfbasic \<alpha>''" using 3(4,5) fwd_wfbasic by blast
+  hence "inter\<^sub>c (step\<^sub>t R) (step G) c\<^sub>2 \<alpha>" using 3 rif_checks_postfix by fastforce
+  moreover have "inter\<^sub>c (step\<^sub>t R) (step G) c\<^sub>1 \<alpha>''" 
+    using \<alpha> 3(1)[OF 3(3) _ w _ \<alpha>(1)] 3(4,6,8)
+    using  rif_checks_fwd[OF \<alpha>(2) _ 3(5), of c\<^sub>1]  by simp
+  ultimately show ?case using \<alpha> by auto
+next
+  case (4 \<alpha>' c\<^sub>1 c\<^sub>2 \<alpha>)
+  then obtain \<alpha>'' where \<alpha>: "reorder_com \<alpha>' c\<^sub>1 \<alpha>''" "reorder_com \<alpha>'' c\<^sub>2 \<alpha>" by auto
+  hence w:  "wfbasic \<alpha>''" using 4(4,5) fwd_wfbasic by blast
+  hence "inter\<^sub>c (step\<^sub>t R) (step G) c\<^sub>2 \<alpha>" using 4 rif_checks_postfix by fastforce
+  moreover have "inter\<^sub>c (step\<^sub>t R) (step G) c\<^sub>1 \<alpha>''" 
+    using \<alpha> 4(1)[OF 4(3) _ w _ \<alpha>(1)] 4(4,6,8)
+    using  rif_checks_fwd[OF \<alpha>(2) _ 4(5), of c\<^sub>1]  by simp
+  ultimately show ?case using \<alpha> by auto
+qed auto 
+
+text \<open>rif should perform checks on any instruction that can reorder before some prefix\<close>
+lemma exec_rif_checks:
+  assumes "wellformed R G" "wfcom r" "wfbasic \<alpha>" "sim r"
+  assumes "lexecute c r \<alpha> c'"
+  assumes "checks (rif (r ;; Basic \<alpha>) {}) R G"
+  shows "inter\<^sub>c (step\<^sub>t R) (step G) r \<alpha>"
+  using assms exec_to_reorder exec_checks_induct by blast
+
+subsection \<open>Remaining rif Checks\<close>
+
+text \<open>
+It is necessary to show that the early execution of an instruction does not result in
+a remaining program for which rif no longer holds. 
+We demonstrate this by relating two versions of the analysis, one where the executed
+instruction has been considered and one where it is not.
+We then demonstrate that checks against the version with the instruction present imply
+those where it is not.
+\<close>
+
+text \<open>
+Compare two points ignoring the implications of some instruction \<alpha>,
+such that the checks of the LHS are implied by those of the RHS and the
+reordering constraints of the LHS are stronger than the RHS ignoring \<alpha>.
+\<close>
+definition point_ign :: "('v,'r,'a) point \<Rightarrow> (_,_,_) subbasic \<Rightarrow> (_,_,_) point \<Rightarrow> bool" 
+  ("_ \<sim>\<^sub>_ _" [0,100,0] 60)
+  where "point_ign p \<alpha> q \<equiv> 
+     wrs p \<subseteq> wrs q \<union> wr (inst \<alpha>) \<and> 
+     rds p \<subseteq> rds q \<union> (wrs q - locals) \<union> rd (inst \<alpha>) \<and> 
+     (bar p \<subseteq> bar q \<union> (if hasGlobal (wrs q) then {cfence} else {}) \<union> barriers (inst \<alpha>)) \<and>
+     (op p = op q) \<and>
+     (esc p = esc q) \<and>
+     (pairs p \<supseteq> pairs q)"
+
+lemma [intro]:
+  "p \<sim>\<^sub>\<alpha> p"
+  by (auto simp: point_ign_def)
+
+text \<open>
+Extend the point comparison over two sets of points, such that there exists a point in
+the RHS for all in the LHS.
+\<close>
+definition points_ign :: "('v,'r,'a) points \<Rightarrow> (_,_,_) subbasic \<Rightarrow> (_,_,_) points \<Rightarrow> bool"
+  ("_ \<approx>\<^sub>_ _" [0,100,0] 60)
+  where "points_ign P \<alpha> Q \<equiv> \<forall>q \<in> Q. \<exists>p \<in> P. (p \<sim>\<^sub>\<alpha> q)"
+
+text \<open>
+Given an instruction that the ignored operation can reorder before, q should have
+stronger reordering constraints than p.
+\<close>
+lemma point_ign_ord:
+  assumes "reorder_inst \<alpha>' \<beta> \<alpha>" "inst \<beta> \<noteq> cfence"
+  assumes "p \<sim>\<^sub>\<alpha> q"
+  shows "ord (inst \<beta>) p \<longrightarrow> ord (inst \<beta>) q"
+proof (cases \<beta> rule: opbasicE)
+  case (op x e f v b)
+  then show ?thesis by (insert assms, cases \<alpha> rule: opbasicE; 
+      clarsimp simp: point_ign_def hasGlobal_def split: if_splits; blast)
+next
+  case (cmp g f v b)
+  then show ?thesis by (insert assms, cases \<alpha> rule: opbasicE; 
+      clarsimp simp: point_ign_def hasGlobal_def split: if_splits; blast)
+next
+  case (fence f v b)
+  then show ?thesis by (insert assms, cases \<alpha> rule: opbasicE; 
+    clarsimp simp: point_ign_def hasGlobal_def split: if_splits; blast)
+next
+  case (cfence f v b)
+  then show ?thesis by (insert assms, cases \<alpha> rule: opbasicE; 
+    clarsimp simp: point_ign_def hasGlobal_def split: if_splits; blast)
+next
+  case (stfence f v b)
+  then show ?thesis by (insert assms, cases \<alpha> rule: opbasicE; 
+    clarsimp simp: point_ign_def hasGlobal_def split: if_splits; blast)
+next
+  case (load x e f v b)
+  then show ?thesis by (insert assms, cases \<alpha> rule: opbasicE; 
+    clarsimp simp: point_ign_def hasGlobal_def split: if_splits; blast)
+next
+  case (store x e f v b)
+  then show ?thesis by (insert assms, cases \<alpha> rule: opbasicE; 
+    clarsimp simp: point_ign_def hasGlobal_def split: if_splits; blast)
+next
+  case (cas\<^sub>T x e1 e2 f v b)
+  then show ?thesis by (insert assms, cases \<alpha> rule: opbasicE; 
+    clarsimp simp: point_ign_def hasGlobal_def split: if_splits; blast)
+next
+  case (cas\<^sub>F x e1 f v b)
+  then show ?thesis by (insert assms, cases \<alpha> rule: opbasicE; 
+    clarsimp simp: point_ign_def hasGlobal_def split: if_splits; blast)
+next
+  case (nop f v b)
+  then show ?thesis by (insert assms, cases \<alpha> rule: opbasicE; 
+    clarsimp simp: point_ign_def hasGlobal_def split: if_splits; blast)
+qed
+
+text \<open>
+The point_ign relation is preserved across updates due to an instruction that the
+ignored instruction can reorder before.
+\<close>
+lemma point_ign_pres:
+  assumes "reorder_inst \<alpha>' \<beta> \<alpha>" "p \<sim>\<^sub>\<alpha> q" "q' \<in> proc1 \<beta> q"
+  shows "\<exists>p'\<in>proc1 \<beta> p. (p' \<sim>\<^sub>\<alpha>' q')"
+proof (cases "q' = stren \<beta> q")
+  case True
+  moreover have "stren \<beta> p \<sim>\<^sub>\<alpha>' (stren \<beta> q)" 
+    using assms(1,2) by (auto simp: stren_def point_ign_def hasGlobal_def split: if_splits)
+  ultimately show ?thesis by blast
+next
+  case False
+  text \<open>Must have weakened due to out-of-order otherwise\<close>
+  hence q: "q' = wken \<beta> q" "\<not> ord (inst \<beta>) q" 
+    using assms(3) unfolding proc1_def by (auto split: if_splits)
+  text \<open>Therefore, \<beta> can't have a global write in common with q\<close>
+  hence wr: "(wr (inst \<beta>) - locals) \<inter> wrs q = {}"
+    by (cases "inst \<beta>"; auto split: var.splits)
+
+  show ?thesis
+  proof (cases "inst \<beta> = cfence")
+    case True
+    hence "fence \<notin> barriers (inst \<alpha>) \<and> rd (inst \<alpha>) \<subseteq> locals"
+      using assms(1) by (cases \<alpha> rule: opbasicE; cases \<beta> rule: opbasicE) auto
+    hence "ord (inst \<beta>) p \<Longrightarrow> (stren \<beta> p) \<sim>\<^sub>\<alpha>' (wken \<beta> q)"
+      using assms(1,2) q(2) by (auto simp: hasGlobal_def True stren_def wken_def point_ign_def)
+    moreover have "\<not>ord (inst \<beta>) p \<Longrightarrow> wken \<beta> p \<sim>\<^sub>\<alpha>' (wken \<beta> q)"
+      using assms(1,2) q(2) by (auto simp: True wken_def point_ign_def)
+    ultimately show ?thesis using q(1) unfolding proc1_def by auto
+  next
+    case False
+    text \<open>Also, \<beta> can't be ordered with p due to q's stronger constraints\<close>
+    hence "\<not> ord (inst \<beta>) p" using q point_ign_ord assms(1,2) by blast
+    text \<open>Therefore, \<beta> must weaken p as well\<close>
+    hence "wken \<beta> p \<in> proc1 \<beta> p" unfolding proc1_def by auto
+    text \<open>wken preserves the relation\<close>
+    moreover have "wken \<beta> p \<sim>\<^sub>\<alpha>' (wken \<beta> q)"
+      using assms(1,2) wr unfolding wken_def point_ign_def
+      apply (intro conjI)
+      apply (clarsimp; blast)+
+      by (auto split: subop.splits)
+    ultimately show ?thesis using q(1) by blast
+  qed
+qed
+
+text \<open>
+It is possible to establish the points_ign relation between P and a version of P
+updated using the ignored instruction.
+\<close>
+lemma points_ignI [intro]:
+  shows "rif (Basic \<alpha>) P \<approx>\<^sub>\<alpha> P"
+proof (simp add: points_ign_def rif\<^sub>i_def, intro ballI disjI2)
+  fix q assume "q \<in> P"
+  moreover have "stren \<alpha> q \<sim>\<^sub>\<alpha> q" by (auto simp: stren_def point_ign_def)
+  ultimately show "\<exists>y\<in>P. \<exists>p\<in>proc1 \<alpha> y. (p \<sim>\<^sub>\<alpha> q)" by auto
+qed
+
+text \<open>
+It is also possible to preserve the points_ign relation across a program that
+the ignored instruction can reorder before.
+\<close>
+lemma points_ign_presI [intro]:
+  assumes "reorder_com \<beta> r \<alpha>" "sim r"
+  assumes "P \<approx>\<^sub>\<alpha> Q"
+  shows "rif r P \<approx>\<^sub>\<beta> (rif r Q)"
+  using assms
+proof (induct \<beta> r \<alpha> arbitrary: P Q rule: reorder_com.induct)
+  case (2 \<alpha>' \<beta> \<alpha>)
+  then show ?case using point_ign_pres by (simp add: rif\<^sub>i_def points_ign_def) blast
+qed auto
+
+text \<open>
+Checks against the RHS of the points_ign relation implies checks against the LHS.
+\<close>
+lemma points_ign_check:
+  assumes "P \<approx>\<^sub>\<alpha> Q"
+  assumes "checks P R G"
+  shows "checks Q R G"
+proof (simp add: checks_def, intro ballI)
+  fix q \<beta> assume q: "q \<in> Q" "\<beta> \<in> pairs q"
+  then obtain p where p: "p \<in> P" "p \<sim>\<^sub>\<alpha> q" using assms(1) by (auto simp: points_ign_def)
+  hence "\<beta> \<in> pairs p" "op p = op q" using q by (auto simp: point_ign_def)
+  thus "chke \<beta> (op q) R G" using p(1) assms(2) by (auto simp: checks_def)
+qed
+
+text \<open>
+These properties allow us to show that rif checks for (r ;; \<alpha>) imply the rif checks for 
+just r given \<alpha> can execute before r. 
+\<close>
+theorem remaining_rif_checks:
+  assumes "lexecute c r \<alpha> c'" "sim r"
+  assumes "checks (rif (r ;; Basic \<alpha>) P) R G"
+  shows "checks (rif r P) R G"
+proof -
+  obtain \<alpha>' where "reorder_com \<alpha>' r \<alpha>" using assms(1) exec_to_reorder by metis
+  moreover have "rif (Basic \<alpha>) P \<approx>\<^sub>\<alpha> P" by blast
+  ultimately have i: "rif r (rif (Basic \<alpha>) P) \<approx>\<^sub>\<alpha>' (rif r P)"
+    using points_ign_presI assms(2) by fastforce
+  thus ?thesis using assms(3) points_ign_check by simp blast
+qed
+
+subsection \<open>Soundness\<close>
+
+text \<open>
+Show that the rif analysis can be rephrased in terms of the prefix r and instruction \<alpha>
+encountered when executing a program step.
+\<close>
+lemma rif_lexecute:
+  assumes "lexecute c r \<alpha> c'" 
+  shows "\<exists>c\<^sub>2. rif c P = rif ((r ;; Basic \<alpha>) ;; c\<^sub>2) P \<and> rif c' P = rif (r ;; c\<^sub>2) P"
+  using assms
+proof (induct arbitrary: P)
+  case (act \<alpha>)
+  have a: "rif\<^sub>i \<alpha> P = rif\<^sub>i \<alpha> (rif Nil P)" "P = rif Nil P" by auto
+  show ?case apply auto using a by blast
+next
+  case (ino c\<^sub>1 r \<alpha> c\<^sub>1' c\<^sub>2)
+  then obtain c where 
+    "rif (c\<^sub>1 ;; c\<^sub>2) P = rif ((r ;; Basic \<alpha>) ;; c ;; c\<^sub>2) P" 
+    "rif (c\<^sub>1' ;; c\<^sub>2) P = rif (r ;; c ;; c\<^sub>2) P"
+    by force
+  then show ?case by blast
+next
+  case (ooo c\<^sub>1 r \<alpha> c\<^sub>1' \<alpha>' c\<^sub>2)
+  then obtain c where "rif c\<^sub>1 P = rif ((r ;; Basic \<alpha>) ;; c) P" "rif c\<^sub>1' P = rif (r ;; c) P" 
+    by force
+  then show ?case by auto
+next
+  case (ord c\<^sub>1 r \<alpha> c\<^sub>1' c\<^sub>2)
+  then obtain c where 
+    "rif (c\<^sub>1 \<cdot> c\<^sub>2) P = rif ((r ;; Basic \<alpha>) ;; c ;; c\<^sub>2) P" 
+    "rif (c\<^sub>1' \<cdot> c\<^sub>2) P = rif (r ;; c ;; c\<^sub>2) P"
+    by force
+  then show ?case by blast
+qed 
+
+text \<open>
+Soundness statement suitable for induction over the reordering trace property.
+Reordering trace consists of steps of rewrites and program steps, which we verify separately.
+\<close>
+lemma rif_sound_induct:
+  assumes "reorder_trace t c" "sim c" "wfcom c"
+  assumes "wellformed R G" "checks (rif c {}) R G"
+  shows "\<forall>(r,\<alpha>) \<in> set t. inter\<^sub>c (step\<^sub>t R) (step G) r \<alpha>"
+  using assms
+proof (induct)
+  case (1 c)
+  then show ?case by auto
+next
+  case (2 c c' t)
+  thus ?case using silent_rif_checks sim_silent wfcom_silent 
+    unfolding checks_def by fast
+next
+  case (3 c r \<alpha> c' t)
+  text \<open>Re-phrase rif in terms of r and \<alpha>\<close>
+  then obtain c\<^sub>2 where c2[simp]: 
+      "rif c {} = rif ((r ;; Basic \<alpha>) ;; c\<^sub>2) {}" "rif c' {} = rif (r ;; c\<^sub>2) {}"
+    using rif_lexecute by metis
+  have s: "sim r" using 3 sim_prefix by blast
+  text \<open>rif checks between r and \<alpha> must have been carried out\<close>
+  have a: "wfcom r \<and> wfbasic \<alpha>" using 3 wfcom_exec_prefix by metis
+  hence "inter\<^sub>c (step\<^sub>t R) (step G) r \<alpha>"
+    using s 3 exec_rif_checks unfolding c2
+    using rif_checks_prefix by (metis rif.simps(4))
+  text \<open>rif checks on the remaining program must have been carried out\<close>
+  moreover have "\<forall>a\<in>set t. case a of (a, b) \<Rightarrow> inter\<^sub>c (step\<^sub>t R) (step G) a b"
+    using 3 by (simp add: remaining_rif_checks[OF _ s] wfcom_exec sim_execute)
+  ultimately show ?case by simp
+qed
+
+text \<open>Simplify the soundness property\<close>
+theorem rif_lift_sound:
+  assumes "checks (rif c {}) R G" "sim c" "wellformed R G" "wfcom c"
+  shows "ARMv8_Rules.rif (step\<^sub>t R) (step G) c"
+  using assms rif_sound_induct unfolding rif_def by blast
+
+theorem rif_sound:
+  assumes "checks (rif (lift\<^sub>c c) {}) R G" "wellformed R G"
+  shows "ARMv8_Rules.rif (step\<^sub>t R) (step G) (lift\<^sub>c c)"
+  using assms by (intro rif_lift_sound) auto
+
+abbreviation rif_checks
+  where "rif_checks c R G \<equiv> checks (rif (lift\<^sub>c c) {}) R G"
+
+end
