ARMv8/ARMv8_Syntax.thy
@@ -1,0 +1,244 @@
+theory ARMv8_Syntax
+  imports ARMv8_Rules
+begin
+
+datatype register = r\<^sub>0 | r\<^sub>1 | r\<^sub>2 | r\<^sub>3 | r\<^sub>4 | r\<^sub>5
+
+syntax
+  "_quote"     :: "'b \<Rightarrow> ('a \<Rightarrow> 'b)"                ("(\<guillemotleft>_\<guillemotright>)" [0] 1000)
+  "_antiquote" :: "('a \<Rightarrow> 'b) \<Rightarrow> 'b"                ("\<acute>_" [1000] 1000)
+  "_Assert"    :: "'a \<Rightarrow> 'a set"                    ("(\<llangle>_\<rrangle>)" [0] 1000)
+
+translations
+  "\<llangle>b\<rrangle>" \<rightharpoonup> "CONST Collect \<guillemotleft>b\<guillemotright>"
+
+parse_translation \<open>
+  let
+    fun quote_tr [t] = Syntax_Trans.quote_tr \<^syntax_const>\<open>_antiquote\<close> t
+      | quote_tr ts = raise TERM ("quote_tr", ts);
+  in [(\<^syntax_const>\<open>_quote\<close>, K quote_tr)] end
+\<close>
+
+type_synonym ('v,'r,'a) thread = "(('v,'a) grel \<times> ('v,'a) grel \<times> ('v,'r,'a) pred \<times> ('v,'r,'a) pred \<times> ('v,'r,'a) com_armv8 \<times> ('v,'r,'a) pred)"
+type_synonym ('v,'r,'a) threads = "('v,'r,'a) thread list"
+
+definition addI
+  where "addI I \<equiv> \<lambda>x. x ! 0 + I"
+
+definition subI
+  where "subI I \<equiv> \<lambda>x. x ! 0 - I"
+
+definition addR
+  where "addR \<equiv> \<lambda>x. x ! 0 + x ! 1"
+
+definition subR
+  where "subR \<equiv> \<lambda>x. x ! 0 - x ! 1"
+
+definition modI
+  where "modI I \<equiv> \<lambda>x. x ! 0 mod I"
+
+definition modR
+  where "modR \<equiv> \<lambda>x. x ! 0 mod x ! 1"
+
+definition movI
+  where "movI I \<equiv> \<lambda>x. I"
+
+definition ODD :: "'b \<Rightarrow> ((nat,'b) exp \<times> (nat \<Rightarrow> nat \<Rightarrow> bool) \<times> (nat,'b) exp)"
+  where "ODD r = (Exp (\<lambda>x. x ! 0 mod 2) [Var r], (=), Val 1)"
+
+definition NEQ :: "'b \<Rightarrow> 'b \<Rightarrow> ((nat,'b) exp \<times> (nat \<Rightarrow> nat \<Rightarrow> bool) \<times> (nat,'b) exp)"
+  where "NEQ r1 r2 = (Var r1, (\<noteq>), Var r2)"
+
+definition LE :: "'b \<Rightarrow> 'b \<Rightarrow> ((nat,'b) bexp)"
+  where "LE r1 r2 = Exp\<^sub>B (\<lambda>x. x!0 < x!1) [Var r1, Var r2]"
+
+definition Z ::  "'b \<Rightarrow> ((nat,'b) bexp)"
+  where "Z r = Exp\<^sub>B (\<lambda>x. x!0 = 0) [Var r]"
+
+syntax
+  "_Load"  :: "'r \<Rightarrow> 'r \<Rightarrow> ('v,'r,'a) com_armv8" ("(_ := [_])" [70, 65] 61)
+  "_LoadC"  :: "'r \<Rightarrow> 'r \<Rightarrow> 'c \<Rightarrow> ('v,'r,'a) com_armv8" ("(_ := [_ + #_])" [70, 65] 61)
+  "_LoadIC"  :: "('v,'r,'a) pred \<Rightarrow> 'r \<Rightarrow> 'r \<Rightarrow> 'c \<Rightarrow> ('v,'r,'a) com_armv8" ("(\<lbrace>_\<rbrace> _ := [_ + #_])" [20, 70, 65] 61)
+
+  "_Store" :: "'r \<Rightarrow> 'r \<Rightarrow> ('v,'r,'a) com_armv8" ("([_] := _)" [70, 65] 61)
+  "_StoreI" :: "('v,'r,'a) pred \<Rightarrow> 'r \<Rightarrow> 'v \<Rightarrow> 'r \<Rightarrow> ('v,'r,'a) com_armv8" ("(\<lbrace>_\<rbrace> [_ + #_] := _)" [20, 70, 65] 61)
+  "_StoreIA" :: "('v,'r,'a) pred \<Rightarrow> 'r \<Rightarrow> 'v \<Rightarrow> 'r \<Rightarrow> ('v,'r,'a) auxfn  \<Rightarrow> ('v,'r,'a) com_armv8" ("(\<lbrace>_\<rbrace> [_ + #_] := _ :\<^sub>a _)" [20, 70, 65] 61)
+  
+  "_Fence" :: "(nat,'b,'a) com_armv8" ("(fence)" 61)
+  "_CFence" :: "(nat,'b,'a) com_armv8" ("(cfence)" 61)
+  "_Cas" :: "('v,'r,'a) pred \<Rightarrow> 'r \<Rightarrow> 'r \<Rightarrow> 'r \<Rightarrow> 'r \<Rightarrow> ('v,'r,'a) auxfn  \<Rightarrow> ('v,'b,'a) com_armv8" ("(\<lbrace>_\<rbrace> _ := cas _ _ _, _)" [20, 70, 65] 61)
+
+  "_AddI"  :: "'b \<Rightarrow> 'b \<Rightarrow> nat \<Rightarrow> (nat,'b,'a) com_armv8" ("(_ := _ + #_)" [70, 65, 65] 61)
+  "_SubI"  :: "'b \<Rightarrow> 'b \<Rightarrow> nat \<Rightarrow> (nat,'b,'a) com_armv8" ("(_ := _ - #_)" [70, 65, 65] 61)
+
+  "_AddR"  :: "'b \<Rightarrow> 'b \<Rightarrow> 'b \<Rightarrow> (nat,'b,'a) com_armv8" ("(_ := _ + _)" [70, 65, 65] 61)
+  "_SubR"  :: "'b \<Rightarrow> 'b \<Rightarrow> 'b \<Rightarrow> (nat,'b,'a) com_armv8" ("(_ := _ - _)" [70, 65, 65] 61)
+
+  "_ModI"  :: "'b \<Rightarrow> 'b \<Rightarrow> nat \<Rightarrow> (nat,'b,'a) com_armv8" ("(_ := _ % #_)" [70, 65, 65] 61)
+  "_ModR"  :: "'b \<Rightarrow> 'b \<Rightarrow> 'b \<Rightarrow> (nat,'b,'a) com_armv8" ("(_ := _ % _)" [70, 65, 65] 61)
+  "_MovI"  :: "'b \<Rightarrow> nat \<Rightarrow> (nat,'b,'a) com_armv8" ("(_ := #_)" [70, 65] 61)
+  "_Seq"   :: "(nat,'b,'a) com_armv8 \<Rightarrow> (nat,'b,'a) com_armv8 \<Rightarrow> (nat,'b,'a) com_armv8" ("(_;/ _)" [60,61] 60)
+
+  "_If" :: "((nat,'b) exp \<times> (nat \<Rightarrow> nat \<Rightarrow> bool) \<times> (nat,'b) exp) \<Rightarrow> (nat,'b,'a) com_armv8 \<Rightarrow> (nat,'b,'a) com_armv8 \<Rightarrow> (nat,'b,'a) com_armv8" 
+                ("(if _/ then _ //else _ /fi)"   [0,0,0] 61)
+  "_If1" :: "'b \<Rightarrow> ('v,'r,'a) com_armv8 \<Rightarrow> ('v,'r,'a) com_armv8" 
+                ("(if _/ then _ /fi)"   [0,0] 61)
+  "_Spec" :: "('v,'a) grel \<Rightarrow> ('v,'a) grel \<Rightarrow> ('v,'r,'a) pred \<Rightarrow> ('v,'r,'a) pred \<Rightarrow> ('v,'r,'a) com_armv8 \<Rightarrow> ('v,'r,'a) pred \<Rightarrow> ('v,'r,'a) thread"
+                ("(R: _ //G:_ //I: _ //P: _ //{ _ } //Q: _)" [0,0,0,0] 61)
+  "_AuxAssign"    :: "idt \<Rightarrow> 'b \<Rightarrow> ('v,'r,'a) auxfn" ("(\<^sup>a_ :=/ _)" [70, 65] 61)
+
+translations
+  "\<^sup>ax := a" \<rightharpoonup> "CONST state_rec.more o \<guillemotleft>\<acute>(state_rec.more_update (_update_name x (\<lambda>_. a)))\<guillemotright>"
+
+  "x := [a]" \<rightharpoonup> "CONST Load (CONST UNIV) (CONST Reg a) x (CONST state_rec.more)"
+  "x := [a + #I]" \<rightharpoonup> "CONST Load (CONST UNIV) (CONST Exp (CONST addI I) [CONST Reg a]) x (CONST state_rec.more)"
+  "\<lbrace>P\<rbrace> x := [a + #I]" \<rightharpoonup> "CONST Load \<llangle>P\<rrangle> (CONST Exp (CONST addI I) [CONST Reg a]) x (CONST state_rec.more)"
+
+  "[a] := r" \<rightharpoonup> "CONST Store (CONST UNIV) (CONST Reg a) r (CONST state_rec.more)"
+  "\<lbrace>P\<rbrace> [a + #I] := x" \<rightharpoonup> "CONST Store \<llangle>P\<rrangle> (CONST Exp (CONST addI I) [CONST Reg a]) x (CONST state_rec.more)"
+  "\<lbrace>P\<rbrace> [ra + #I] := r :\<^sub>a a" \<rightharpoonup> "CONST Store \<llangle>P\<rrangle> (CONST Exp (CONST addI I) [CONST Reg ra]) r a"
+
+  "\<lbrace>P\<rbrace> r\<^sub>1 := cas r\<^sub>2 r\<^sub>3 r\<^sub>4, a" \<rightharpoonup> "CONST CAS \<llangle>P\<rrangle> r\<^sub>2 r\<^sub>3 r\<^sub>4 r\<^sub>1 1 0 a"
+
+  "X := Y - #I" \<rightharpoonup> "CONST Op X (CONST Exp (CONST subI I) [CONST Reg Y])"
+  "X := Y + #I" \<rightharpoonup> "CONST Op X (CONST Exp (CONST addI I) [CONST Reg Y])"
+  "X := Y + Z" \<rightharpoonup> "CONST Op X (CONST Exp (CONST addR) [CONST Reg Y, CONST Reg Z])"
+  "X := Y - Z" \<rightharpoonup> "CONST Op X (CONST Exp (CONST subR) [CONST Reg Y, CONST Reg Z])"
+  "X := Y % #I" \<rightharpoonup> "CONST Op X (CONST Exp (CONST modI I) [CONST Reg Y])"
+  "X := Y % Z" \<rightharpoonup> "CONST Op X (CONST Exp (CONST modR) [CONST Reg Y, CONST Reg Z])"
+
+  "X := #I" \<rightharpoonup> "CONST Op X (CONST Exp (CONST movI I) [])"
+  "fence" \<rightharpoonup> "CONST Fence"
+  "cfence" \<rightharpoonup> "CONST Fence"
+  "c\<^sub>1 ; c\<^sub>2" \<rightharpoonup> "CONST Seq c\<^sub>1 c\<^sub>2"
+  "if b then c\<^sub>1 else c\<^sub>2 fi" \<rightharpoonup> "CONST If b c\<^sub>1 c\<^sub>2"
+  "if b then c\<^sub>1 fi" \<rightharpoonup> "CONST If b c\<^sub>1 (CONST Skip)"
+  "R: R G: G I: I P: P {c} Q: Q" \<rightharpoonup> "(\<llangle>R\<rrangle>,\<llangle>G\<rrangle>,\<llangle>I\<rrangle>,\<llangle>P\<rrangle>,c,\<llangle>Q\<rrangle>)"
+
+definition inv2
+  where "inv2 I \<equiv> {(m,m'). m \<in> glb ` I \<longrightarrow> m' \<in> glb ` I}"
+
+definition rif_checks
+  where "rif_checks c R G = True"
+
+fun fn_valid :: "('v::equal,'r::equal,'a) threads \<Rightarrow> bool"
+  where 
+    "fn_valid [(R,G,I,P,c,Q)] = (stable\<^sub>t R Q \<and> wellformed R G \<and> guar\<^sub>c c (inv2 I \<inter> G) \<and> 
+                                (wellformed R G \<longrightarrow> stable\<^sub>t R Q \<longrightarrow> P \<subseteq> wp R c Q) \<and>
+                                (wellformed R G \<longrightarrow> rif_checks c R G))" |
+    "fn_valid _ = undefined"
+
+nonterminal prgs
+
+syntax
+  "_PAR"        :: "prgs \<Rightarrow> 'a"              ("COBEGIN//_//COEND" 60)
+  "_FN"        :: "prgs \<Rightarrow> 'a"              ("FNBEGIN//_//FNEND" 60)
+  "_prg"        :: "'a \<Rightarrow> prgs"              ("_" 57)
+  "_prgs"       :: "['a, prgs] \<Rightarrow> prgs"      ("_//\<parallel>//_" [60,57] 57)
+
+translations
+  "_prg a" \<rightharpoonup> "[a]"
+  "_prgs a ps" \<rightharpoonup> "a # ps"
+  "_FN t" \<rightharpoonup> "CONST fn_valid t"
+
+syntax
+  "_before"  :: "'b \<Rightarrow> 'a" ("\<^sup>1_" [100] 400)
+  "_after"   :: "'b \<Rightarrow> 'a" ("\<^sup>2_" [100] 400)
+  "_mem"     :: "nat \<Rightarrow> 'a" ("\<^sup>s[_]")
+  "_mbefore" :: "nat \<Rightarrow> 'a" ("\<^sup>1[_]")
+  "_mafter"  :: "nat \<Rightarrow> 'a" ("\<^sup>2[_]")
+  "_reg"     :: "'r \<Rightarrow> 'a" ("\<^sup>r_" [100] 1000)
+  "_rbefore" :: "'r \<Rightarrow> 'a" ("\<^sup>1\<^sup>r_")
+  "_rafer"   :: "'r \<Rightarrow> 'a" ("\<^sup>2\<^sup>r_")
+  "_aux"     :: "'b \<Rightarrow> 'a" ("\<^sup>a_" [100] 1000)
+  "_abefore" :: "'b \<Rightarrow> 'a" ("\<^sup>1\<^sup>a_" [100] 400)
+  "_aafer"   :: "'b \<Rightarrow> 'a" ("\<^sup>2\<^sup>a_" [100] 400)
+
+translations
+  "\<^sup>1x" \<rightleftharpoons> "x (\<acute>CONST fst)"
+  "\<^sup>2x" \<rightleftharpoons> "x (\<acute>CONST snd)"
+  "\<^sup>s[X]" \<rightleftharpoons> "(\<acute>CONST st) X"
+  "\<^sup>1[X]" \<rightleftharpoons> "(CONST st (\<acute>CONST fst)) X"
+  "\<^sup>2[X]" \<rightleftharpoons> "(CONST st (\<acute>CONST snd)) X"
+  "\<^sup>rX" \<rightleftharpoons> "(\<acute>CONST rg) X"
+  "\<^sup>1\<^sup>rX" \<rightleftharpoons> "(CONST rg (\<acute>CONST fst)) X"
+  "\<^sup>2\<^sup>rX" \<rightleftharpoons> "(CONST rg (\<acute>CONST snd)) X"
+  "\<^sup>aX" \<rightleftharpoons> "X (\<acute>CONST state_rec.more)"
+  "\<^sup>1\<^sup>aX" \<rightleftharpoons> "X (CONST state_rec.more (\<acute>CONST fst))"
+  "\<^sup>2\<^sup>aX" \<rightleftharpoons> "X (CONST state_rec.more (\<acute>CONST snd))"
+
+(*
+syntax
+  "_before"  :: "'b \<Rightarrow> 'a" ("\<^sup>1_" [100] 400)
+  "_after"   :: "'b \<Rightarrow> 'a" ("\<^sup>2_" [100] 400)
+  "_mem"     :: "'b \<Rightarrow> 'a" ("\<lbrakk>_\<rbrakk>")
+  "_mat"     :: "'b \<Rightarrow> 'a" ("\<^sup>0\<lbrakk>_\<rbrakk>")
+  "_mbefore" :: "'b \<Rightarrow> 'a" ("\<^sup>1\<lbrakk>_\<rbrakk>")
+  "_mafter"  :: "'b \<Rightarrow> 'a" ("\<^sup>2\<lbrakk>_\<rbrakk>")
+  "_reg"     :: "'r \<Rightarrow> 'a" ("\<^bold>r_" [1000] 1000)
+  "_rar"     :: "'r \<Rightarrow> 'a" ("\<^sup>0\<^bold>r_" [100] 1000)
+  "_rbefore" :: "'r \<Rightarrow> 'a" ("\<^sup>1\<^bold>r_")
+  "_rafer"   :: "'r \<Rightarrow> 'a" ("\<^sup>2\<^bold>r_")
+  "_val"     :: "'b \<Rightarrow> 'a" ("#_" [100] 1000)
+  "_aux"     :: "'b \<Rightarrow> 'a" ("\<^sup>a_" [100] 1000)
+  "_abefore" :: "'b \<Rightarrow> 'a" ("\<^sup>1\<^sup>a_" [100] 400)
+  "_aafer"   :: "'b \<Rightarrow> 'a" ("\<^sup>2\<^sup>a_" [100] 400)
+
+translations
+  "\<^sup>1x" \<rightleftharpoons> "x (\<acute>CONST fst)"
+  "\<^sup>2x" \<rightleftharpoons> "x (\<acute>CONST snd)"
+  "\<lbrakk>X\<rbrakk>" \<rightleftharpoons> "CONST Var (CONST Glb X)"
+  "\<^sup>0\<lbrakk>X\<rbrakk>" \<rightleftharpoons> "(CONST st (\<acute>CONST glb)) X"
+  "\<^sup>1\<lbrakk>X\<rbrakk>" \<rightleftharpoons> "(CONST st (\<acute>CONST fst)) X"
+  "\<^sup>2\<lbrakk>X\<rbrakk>" \<rightleftharpoons> "(CONST st (\<acute>CONST snd)) X"
+  "\<^bold>rX" \<rightleftharpoons> "CONST Var (CONST Reg X)"
+  "\<^sup>0\<^bold>rX" \<rightleftharpoons> "(\<acute>CONST rg) X"
+  "\<^sup>1\<^bold>rX" \<rightleftharpoons> "(CONST rg (\<acute>CONST fst)) X"
+  "\<^sup>2\<^bold>rX" \<rightleftharpoons> "(CONST rg (\<acute>CONST snd)) X"
+  "#X" \<rightleftharpoons> "CONST Val X"
+  "\<^sup>aX" \<rightleftharpoons> "X (\<acute>CONST state_rec.more)"
+  "\<^sup>1\<^sup>aX" \<rightleftharpoons> "X (CONST state_rec.more (\<acute>CONST fst))"
+  "\<^sup>2\<^sup>aX" \<rightleftharpoons> "X (CONST state_rec.more (\<acute>CONST snd))"
+*)
+
+syntax
+  "_con" :: "nat \<Rightarrow> 'a" ("=[_]" [100] 1000)
+  "_inc" :: "nat \<Rightarrow> 'a" ("\<le>[_]" [100] 1000)
+
+translations
+  "=[X]" \<rightharpoonup> "(CONST st (\<acute>CONST snd)) X = (CONST st (\<acute>CONST fst)) X"
+  "\<le>[X]" \<rightharpoonup> "(CONST st (\<acute>CONST snd)) X \<ge> (CONST st (\<acute>CONST fst)) X"
+
+lemma [simp]:
+  "stabilize R UNIV = UNIV"
+  by (auto simp: stabilize_def)
+
+lemma [simp]:
+  "reflexive R \<Longrightarrow> stabilize R {} = {}"
+  by (auto simp: reflexive_def stabilize_def)
+
+lemma [simp]:
+  "reflexive R \<Longrightarrow> stabilize R (assert P) = assert P"
+  by (auto simp: assert_def)
+
+lemma [simp]:
+  "{m. m(a :=\<^sub>s e) \<in> (assert P)} = assert P"
+  by (auto simp: assert_def)
+
+lemma [simp]:
+  "reflexive R \<Longrightarrow> UNIV \<subseteq> stabilize R P = (\<forall>m. m \<in> P)"
+  by (auto simp: reflexive_def stabilize_def assert_def glb_def)
+
+lemma [simp]:
+  "stabilize R (P \<inter> Q) = stabilize R P \<inter> stabilize R Q"
+  by (auto simp: stabilize_def)
+
+lemma [simp]:
+  "{m. (f m) \<in> assert P} = assert P"
+  by (auto simp: assert_def)
+
+lemma [simp]:
+  "UNIV \<subseteq> assert P = P"
+  by (auto simp: assert_def)
+
+end
