Reordering.thy
@@ -23,16 +23,6 @@ abbreviation reorder_inst :: "('a,'b) basic \<Rightarrow> ('a,'b) basic \<Righta
   ("_ < _ <\<^sub>a _" [100,0,100] 100)
   where "\<beta>' < \<alpha> <\<^sub>a \<beta> \<equiv> \<beta>' = \<beta>\<langle>tag \<alpha>\<rangle> \<and> tag \<alpha> \<hookleftarrow> (tag \<beta>\<langle>tag \<alpha>\<rangle>)"
 
-text \<open>Recursively define reordering of an instruction earlier than a program\<close>
-fun reorder_com :: "('a,'b) basic \<Rightarrow> ('a,'b) com \<Rightarrow> ('a,'b) basic \<Rightarrow> bool"
-  ("_ < _ <\<^sub>c _" [100,0,100] 100)
-  where
-    "\<alpha>' < Nil <\<^sub>c \<alpha> = (\<alpha>' = \<alpha>)" |
-    "\<alpha>' < Basic \<beta> <\<^sub>c \<alpha> = (\<alpha>' < \<beta> <\<^sub>a \<alpha>)" |
-    "\<alpha>' < c\<^sub>1 ;; c\<^sub>2 <\<^sub>c \<alpha> = (\<exists>\<alpha>\<^sub>n. \<alpha>' < c\<^sub>1 <\<^sub>c \<alpha>\<^sub>n \<and> \<alpha>\<^sub>n < c\<^sub>2 <\<^sub>c \<alpha>)" |
-    "\<alpha>' < c\<^sub>1 \<cdot> c\<^sub>2 <\<^sub>c \<alpha> = (\<exists>\<alpha>\<^sub>n. \<alpha>' < c\<^sub>1 <\<^sub>c \<alpha>\<^sub>n \<and> \<alpha>\<^sub>n < c\<^sub>2 <\<^sub>c \<alpha>)" |
-    "_ < _ <\<^sub>c _ = False"
-
 text \<open>Recursively define forwarding of an instruction across a program\<close>
 fun fwd_com :: "('a,'b) basic \<Rightarrow> ('a,'b) com \<Rightarrow> ('a,'b) basic"
   ("_\<llangle>_\<rrangle>" [1000,0] 1000)
@@ -42,6 +32,16 @@ fun fwd_com :: "('a,'b) basic \<Rightarrow> ('a,'b) com \<Rightarrow> ('a,'b) ba
     "\<alpha>\<llangle>c\<^sub>1 ;; c\<^sub>2\<rrangle> = \<alpha>\<llangle>c\<^sub>2\<rrangle>\<llangle>c\<^sub>1\<rrangle>" |
     "\<alpha>\<llangle>c\<^sub>1 \<cdot> c\<^sub>2\<rrangle> = \<alpha>\<llangle>c\<^sub>2\<rrangle>\<llangle>c\<^sub>1\<rrangle>" |
     "\<alpha>\<llangle>_\<rrangle> = \<alpha>"
+
+text \<open>Recursively define reordering of an instruction earlier than a program\<close>
+fun reorder_com :: "('a,'b) basic \<Rightarrow> ('a,'b) com \<Rightarrow> ('a,'b) basic \<Rightarrow> bool"
+  ("_ < _ <\<^sub>c _" [100,0,100] 100)
+  where
+    "\<alpha>' < Nil <\<^sub>c \<alpha> = (\<alpha>' = \<alpha>)" |
+    "\<alpha>' < Basic \<beta> <\<^sub>c \<alpha> = (\<alpha>' < \<beta> <\<^sub>a \<alpha>)" |
+    "\<alpha>' < c\<^sub>1 ;; c\<^sub>2 <\<^sub>c \<alpha> = (\<exists>\<alpha>\<^sub>n. \<alpha>' < c\<^sub>1 <\<^sub>c \<alpha>\<^sub>n \<and> \<alpha>\<^sub>n < c\<^sub>2 <\<^sub>c \<alpha>)" |
+    "\<alpha>' < c\<^sub>1 \<cdot> c\<^sub>2 <\<^sub>c \<alpha> = (\<exists>\<alpha>\<^sub>n. \<alpha>' < c\<^sub>1 <\<^sub>c \<alpha>\<^sub>n \<and> \<alpha>\<^sub>n < c\<^sub>2 <\<^sub>c \<alpha>)" |
+    "_ < _ <\<^sub>c _ = False"
 
 text \<open>Relationship between program reordering and program forwarding\<close>
 lemma fwd_com [simp]:
